@prefix : <http://www.is-unit4.org/ontology/EducationalMaterials#> .
@prefix owl: <http://www.w3.org/2002/07/owl#> .
@prefix rdf: <http://www.w3.org/1999/02/22-rdf-syntax-ns#> .
@prefix xml: <http://www.w3.org/XML/1998/namespace> .
@prefix xsd: <http://www.w3.org/2001/XMLSchema#> .
@prefix rdfs: <http://www.w3.org/2000/01/rdf-schema#> .
@base <http://www.is-unit4.org/ontology/EducationalMaterials> .

<http://www.is-unit4.org/ontology/EducationalMaterials> rdf:type owl:Ontology .

#################################################################
#    Annotation properties
#################################################################

###  http://dbpedia.org/ontology/related
<http://dbpedia.org/ontology/related> rdf:type owl:AnnotationProperty .


###  http://www.w3.org/2003/06/sw-vocab-status/ns#term_status
<http://www.w3.org/2003/06/sw-vocab-status/ns#term_status> rdf:type owl:AnnotationProperty .


###  http://www.w3.org/2004/02/skos/core#definition
<http://www.w3.org/2004/02/skos/core#definition> rdf:type owl:AnnotationProperty .


###  http://www.w3.org/2004/02/skos/core#scopeNote
<http://www.w3.org/2004/02/skos/core#scopeNote> rdf:type owl:AnnotationProperty .


###  https://schema.org/inverseOf
<https://schema.org/inverseOf> rdf:type owl:AnnotationProperty .


###  https://schema.org/source
<https://schema.org/source> rdf:type owl:AnnotationProperty .


#################################################################
#    Object Properties
#################################################################

###  http://linkedscience.org/teach/ns#academicTerm
<http://linkedscience.org/teach/ns#academicTerm> rdf:type owl:ObjectProperty ;
                                                 <http://dbpedia.org/ontology/related> <http://dbpedia.org/page/Academic_term> ;
                                                 rdfs:comment "academicTerm is an abstract property to express the academic term (e.g. Summer 2011) of the course/seminar."@en ;
                                                 rdfs:isDefinedBy <http://linkedscience.org/teach/ns#academicTerm> ;
                                                 rdfs:label "academicTerm"@en .


###  http://linkedscience.org/teach/ns#deadline
<http://linkedscience.org/teach/ns#deadline> rdf:type owl:ObjectProperty ;
                                             rdfs:comment "deadline is an abstract property explicate the deadline for a draft project report."@en ;
                                             rdfs:isDefinedBy <http://linkedscience.org/teach/ns#deadline> ;
                                             rdfs:label "deadline"@en .


###  http://linkedscience.org/teach/ns#ects
<http://linkedscience.org/teach/ns#ects> rdf:type owl:ObjectProperty ;
                                         <http://dbpedia.org/ontology/related> <http://dbpedia.org/resource/European_Credit_Transfer_and_Accumulation_System> ;
                                         rdfs:comment "ects is an abstract property to express the ects (European Credit Transfer System) of the course/seminar."@en ;
                                         rdfs:isDefinedBy <http://linkedscience.org/teach/ns#ects> ;
                                         rdfs:label "ects"@en .


###  http://linkedscience.org/teach/ns#grading
<http://linkedscience.org/teach/ns#grading> rdf:type owl:ObjectProperty ;
                                            <http://dbpedia.org/ontology/related> <http://dbpedia.org/resource/Grading> ;
                                            rdfs:comment "grading is an abstract property to relate the course/seminar to the description about its grading."@en ;
                                            rdfs:isDefinedBy <http://linkedscience.org/teach/ns#grading> ;
                                            rdfs:label "grading"@en .


###  http://linkedscience.org/teach/ns#reading
<http://linkedscience.org/teach/ns#reading> rdf:type owl:ObjectProperty ;
                                            rdfs:comment "reading is an abstract property to relate required readings to the course/seminar."@en ;
                                            rdfs:isDefinedBy <http://linkedscience.org/teach/ns#reading> ;
                                            rdfs:label "reading"@en .


###  http://linkedscience.org/teach/ns#studentGroup
<http://linkedscience.org/teach/ns#studentGroup> rdf:type owl:ObjectProperty ;
                                                 rdfs:range <http://xmlns.com/foaf/0.1/Group> ;
                                                 <http://dbpedia.org/ontology/related> <http://dbpedia.org/resource/TEACHER> ;
                                                 rdfs:comment "studentGroup is an abstract property to relate a student group to the course/seminar."@en ;
                                                 rdfs:isDefinedBy <http://linkedscience.org/teach/ns#studentGroup> ;
                                                 rdfs:label "studentGroup"@en .


###  http://linkedscience.org/teach/ns#teacher
<http://linkedscience.org/teach/ns#teacher> rdf:type owl:ObjectProperty ;
                                            <http://dbpedia.org/ontology/related> <http://dbpedia.org/resource/TEACHER> ;
                                            rdfs:comment "teacher is an abstract property to relate a teacher to a course/seminar."@en ;
                                            rdfs:isDefinedBy <http://linkedscience.org/teach/ns#teacher> ;
                                            rdfs:label "teacher"@en .


###  http://linkedscience.org/teach/ns#teacherOf
<http://linkedscience.org/teach/ns#teacherOf> rdf:type owl:ObjectProperty ;
                                              <http://dbpedia.org/ontology/related> <http://dbpedia.org/resource/TEACHER> ;
                                              rdfs:comment "teacherOf is an abstract property to relate a teacher to a course/seminar."@en ;
                                              rdfs:isDefinedBy <http://linkedscience.org/teach/ns#teacherOf> ;
                                              rdfs:label "teacherOf"@en .


###  http://linkedscience.org/teach/ns#weeklyHours
<http://linkedscience.org/teach/ns#weeklyHours> rdf:type owl:ObjectProperty ;
                                                <http://dbpedia.org/ontology/related> <http://de.dbpedia.org/resource/Semesterwochenstunde> ;
                                                rdfs:comment "weeklyHours is an abstract property to express the number of weekly hours for the teaching."@en ;
                                                rdfs:isDefinedBy <http://linkedscience.org/teach/ns#weeklyHours> ;
                                                rdfs:label "weeklyHours"@en .


###  http://ns.inria.fr/semed/eduprogression/v1#hasCourse
<http://ns.inria.fr/semed/eduprogression/v1#hasCourse> rdf:type owl:ObjectProperty ;
                                                       rdfs:domain <http://ns.inria.fr/semed/eduprogression/v1#EKS> ;
                                                       rdfs:range <http://ns.inria.fr/semed/eduprogression/v1#Course> ;
                                                       rdfs:comment "Relates an instance of EKS to an instance of Course."@en ;
                                                       rdfs:isDefinedBy <http://ns.inria.fr/semed/eduprogression#> ;
                                                       rdfs:label "Has course"@en ;
                                                       <http://www.w3.org/2003/06/sw-vocab-status/ns#term_status> "stable" .


###  http://ns.inria.fr/semed/eduprogression/v1#hasEKS
<http://ns.inria.fr/semed/eduprogression/v1#hasEKS> rdf:type owl:ObjectProperty ;
                                                    rdfs:domain <http://ns.inria.fr/semed/eduprogression/v1#Progression> ;
                                                    rdfs:range <http://ns.inria.fr/semed/eduprogression/v1#EKS> ;
                                                    rdfs:comment "Allows a progression to be associated to one or several EKSs."@en ;
                                                    rdfs:isDefinedBy <http://ns.inria.fr/semed/eduprogression#> ;
                                                    rdfs:label "Has an associated EKS "@en ;
                                                    <http://www.w3.org/2003/06/sw-vocab-status/ns#term_status> "stable" .


###  http://ns.inria.fr/semed/eduprogression/v1#hasKnowledge
<http://ns.inria.fr/semed/eduprogression/v1#hasKnowledge> rdf:type owl:ObjectProperty ;
                                                          rdfs:domain <http://ns.inria.fr/semed/eduprogression/v1#EKS> ;
                                                          rdfs:range <http://ns.inria.fr/semed/eduprogression/v1#Knowledge> ;
                                                          rdfs:comment "Relates an instance of EKS to an instance of Knowledge."@en ;
                                                          rdfs:isDefinedBy <http://ns.inria.fr/semed/eduprogression#> ;
                                                          rdfs:label "Has knowledge"@en ;
                                                          <http://www.w3.org/2003/06/sw-vocab-status/ns#term_status> "stable" .


###  http://ns.inria.fr/semed/eduprogression/v1#hasLearningDomain
<http://ns.inria.fr/semed/eduprogression/v1#hasLearningDomain> rdf:type owl:ObjectProperty ;
                                                               rdfs:range <http://ns.inria.fr/semed/eduprogression/v1#LearningDomain> ;
                                                               rdfs:comment "Associates a learning domain to a Progression or to an EKS."@en ;
                                                               rdfs:isDefinedBy <http://ns.inria.fr/semed/eduprogression#> ;
                                                               rdfs:label "Has a learning sub domain"@en ;
                                                               <http://www.w3.org/2003/06/sw-vocab-status/ns#term_status> "stable" .


###  http://ns.inria.fr/semed/eduprogression/v1#hasPointOfReference
<http://ns.inria.fr/semed/eduprogression/v1#hasPointOfReference> rdf:type owl:ObjectProperty ;
                                                                 rdfs:domain <http://ns.inria.fr/semed/eduprogression/v1#EKS> ;
                                                                 rdfs:comment "Relates an instance of EKS to an instance of class PointOfReference."@en ;
                                                                 rdfs:isDefinedBy <http://ns.inria.fr/semed/eduprogression#> ;
                                                                 rdfs:label "Has point of reference"@en ;
                                                                 <http://www.w3.org/2003/06/sw-vocab-status/ns#term_status> "stable" .


###  http://ns.inria.fr/semed/eduprogression/v1#hasRelatedResource
<http://ns.inria.fr/semed/eduprogression/v1#hasRelatedResource> rdf:type owl:ObjectProperty ;
                                                                rdfs:comment "Associates an instance of a class with a resource on DBpedia"@en ;
                                                                rdfs:isDefinedBy <http://ns.inria.fr/semed/eduprogression#> ;
                                                                rdfs:label "Has realted resource on DBpedia"@en ;
                                                                <http://www.w3.org/2003/06/sw-vocab-status/ns#term_status> "stable" .


###  http://ns.inria.fr/semed/eduprogression/v1#hasSkill
<http://ns.inria.fr/semed/eduprogression/v1#hasSkill> rdf:type owl:ObjectProperty ;
                                                      rdfs:domain <http://ns.inria.fr/semed/eduprogression/v1#EKS> ;
                                                      rdfs:range <http://ns.inria.fr/semed/eduprogression/v1#Skill> ;
                                                      rdfs:comment "Relates an instance of EKS to an instance of Skill."@en ;
                                                      rdfs:isDefinedBy <http://ns.inria.fr/semed/eduprogression#> ;
                                                      rdfs:label "Has skill"@en ;
                                                      <http://www.w3.org/2003/06/sw-vocab-status/ns#term_status> "stable" .


###  http://ns.inria.fr/semed/eduprogression/v1#hasVocabularyItem
<http://ns.inria.fr/semed/eduprogression/v1#hasVocabularyItem> rdf:type owl:ObjectProperty ;
                                                               rdfs:domain <http://ns.inria.fr/semed/eduprogression/v1#EKS> ;
                                                               rdfs:range <http://www.w3.org/2004/02/skos/core#Concept> ;
                                                               rdfs:comment "Relates an instance of EKS to an instance of the class VocabularyItem."@en ;
                                                               rdfs:isDefinedBy <http://ns.inria.fr/semed/eduprogression#> ;
                                                               rdfs:label "Has a vocabulary item"@en ;
                                                               <http://www.w3.org/2003/06/sw-vocab-status/ns#term_status> "stable" .


###  http://www.is-unit4.org/ontology/EducationalMaterials#attendsTo
:attendsTo rdf:type owl:ObjectProperty ;
           rdfs:domain <http://linkedscience.org/teach/ns#Student> ;
           rdfs:range <http://linkedscience.org/teach/ns#Lecture> ;
           rdfs:comment "Relates a student and the courses or lessons he or she is attending to"@en ;
           rdfs:label "Attends to"@en .


###  http://www.is-unit4.org/ontology/EducationalMaterials#hasGradingSystem
:hasGradingSystem rdf:type owl:ObjectProperty ;
                  rdfs:domain :Evaluation ;
                  rdfs:range :GradingSystem ;
                  rdfs:comment "Relates an evaluation method with the employed grading system"@en ;
                  rdfs:label "Has grading system"@en .


###  http://www.is-unit4.org/ontology/EducationalMaterials#hasLicense
:hasLicense rdf:type owl:ObjectProperty ;
            rdfs:range :License ;
            rdfs:comment "Relates a creative wor or educational material with its license"@en ;
            rdfs:label "Has license"@en .


###  http://www.w3.org/2004/02/skos/core#broaderTransitive
<http://www.w3.org/2004/02/skos/core#broaderTransitive> rdf:type owl:ObjectProperty ;
                                                        rdfs:subPropertyOf <http://www.w3.org/2004/02/skos/core#semanticRelation> ;
                                                        owl:inverseOf <http://www.w3.org/2004/02/skos/core#narrowerTransitive> ;
                                                        rdf:type owl:TransitiveProperty ;
                                                        rdfs:isDefinedBy <http://www.w3.org/2004/02/skos/core> ;
                                                        rdfs:label "has broader transitive"@en ;
                                                        <http://www.w3.org/2004/02/skos/core#definition> "skos:broaderTransitive is a transitive superproperty of skos:broader." ;
                                                        <http://www.w3.org/2004/02/skos/core#scopeNote> "By convention, skos:broaderTransitive is not used to make assertions. Rather, the properties can be used to draw inferences about the transitive closure of the hierarchical relation, which is useful e.g. when implementing a simple query expansion algorithm in a search application."@en .


###  http://www.w3.org/2004/02/skos/core#hasTopConcept
<http://www.w3.org/2004/02/skos/core#hasTopConcept> rdf:type owl:ObjectProperty ;
                                                    owl:inverseOf <http://www.w3.org/2004/02/skos/core#topConceptOf> .


###  http://www.w3.org/2004/02/skos/core#inScheme
<http://www.w3.org/2004/02/skos/core#inScheme> rdf:type owl:ObjectProperty ;
                                               rdfs:range <http://www.w3.org/2004/02/skos/core#ConceptScheme> ;
                                               rdfs:isDefinedBy <http://www.w3.org/2004/02/skos/core> ;
                                               rdfs:label "is in scheme"@en ;
                                               <http://www.w3.org/2004/02/skos/core#definition> "Relates a resource (for example a concept) to a concept scheme in which it is included."@en ;
                                               <http://www.w3.org/2004/02/skos/core#scopeNote> "A concept may be a member of more than one concept scheme."@en .


###  http://www.w3.org/2004/02/skos/core#mappingRelation
<http://www.w3.org/2004/02/skos/core#mappingRelation> rdf:type owl:ObjectProperty ;
                                                      rdfs:subPropertyOf <http://www.w3.org/2004/02/skos/core#semanticRelation> ;
                                                      rdfs:comment "These concept mapping relations mirror semantic relations, and the data model defined below is similar (with the exception of skos:exactMatch) to the data model defined for semantic relations. A distinct vocabulary is provided for concept mapping relations, to provide a convenient way to differentiate links within a concept scheme from links between concept schemes. However, this pattern of usage is not a formal requirement of the SKOS data model, and relies on informal definitions of best practice."@en ;
                                                      rdfs:isDefinedBy <http://www.w3.org/2004/02/skos/core> ;
                                                      rdfs:label "is in mapping relation with"@en ;
                                                      <http://www.w3.org/2004/02/skos/core#definition> "Relates two concepts coming, by convention, from different schemes, and that have comparable meanings"@en .


###  http://www.w3.org/2004/02/skos/core#narrowerTransitive
<http://www.w3.org/2004/02/skos/core#narrowerTransitive> rdf:type owl:ObjectProperty ;
                                                         rdfs:subPropertyOf <http://www.w3.org/2004/02/skos/core#semanticRelation> ;
                                                         rdf:type owl:TransitiveProperty ;
                                                         rdfs:isDefinedBy <http://www.w3.org/2004/02/skos/core> ;
                                                         rdfs:label "has narrower transitive"@en ;
                                                         <http://www.w3.org/2004/02/skos/core#definition> "skos:narrowerTransitive is a transitive superproperty of skos:narrower." ;
                                                         <http://www.w3.org/2004/02/skos/core#scopeNote> "By convention, skos:narrowerTransitive is not used to make assertions. Rather, the properties can be used to draw inferences about the transitive closure of the hierarchical relation, which is useful e.g. when implementing a simple query expansion algorithm in a search application."@en .


###  http://www.w3.org/2004/02/skos/core#related
<http://www.w3.org/2004/02/skos/core#related> rdf:type owl:ObjectProperty ;
                                              rdfs:subPropertyOf <http://www.w3.org/2004/02/skos/core#semanticRelation> ;
                                              rdf:type owl:SymmetricProperty ;
                                              rdfs:comment "skos:related is disjoint with skos:broaderTransitive"@en ;
                                              rdfs:isDefinedBy <http://www.w3.org/2004/02/skos/core> ;
                                              rdfs:label "has related"@en ;
                                              <http://www.w3.org/2004/02/skos/core#definition> "Relates a concept to a concept with which there is an associative semantic relationship."@en .


###  http://www.w3.org/2004/02/skos/core#semanticRelation
<http://www.w3.org/2004/02/skos/core#semanticRelation> rdf:type owl:ObjectProperty ;
                                                       rdfs:domain <http://www.w3.org/2004/02/skos/core#Concept> ;
                                                       rdfs:range <http://www.w3.org/2004/02/skos/core#Concept> ;
                                                       rdfs:isDefinedBy <http://www.w3.org/2004/02/skos/core> ;
                                                       rdfs:label "is in semantic relation with"@en ;
                                                       <http://www.w3.org/2004/02/skos/core#definition> "Links a concept to a concept related by meaning."@en ;
                                                       <http://www.w3.org/2004/02/skos/core#scopeNote> "This property should not be used directly, but as a super-property for all properties denoting a relationship of meaning between concepts."@en .


###  http://www.w3.org/2004/02/skos/core#topConceptOf
<http://www.w3.org/2004/02/skos/core#topConceptOf> rdf:type owl:ObjectProperty ;
                                                   rdfs:subPropertyOf <http://www.w3.org/2004/02/skos/core#inScheme> ;
                                                   rdfs:domain <http://www.w3.org/2004/02/skos/core#Concept> ;
                                                   rdfs:range <http://www.w3.org/2004/02/skos/core#ConceptScheme> ;
                                                   rdfs:isDefinedBy <http://www.w3.org/2004/02/skos/core> ;
                                                   rdfs:label "is top concept in scheme"@en ;
                                                   <http://www.w3.org/2004/02/skos/core#definition> "Relates a concept to the concept scheme that it is a top level concept of."@en .


###  http://xmlns.com/foaf/0.1/focus
<http://xmlns.com/foaf/0.1/focus> rdf:type owl:ObjectProperty ;
                                  rdfs:domain <http://www.w3.org/2004/02/skos/core#Concept> ;
                                  rdfs:range owl:Thing ;
                                  rdfs:comment "The underlying or 'focal' entity associated with some SKOS-described concept." ;
                                  rdfs:isDefinedBy <http://xmlns.com/foaf/0.1/> ;
                                  rdfs:label "focus" ;
                                  <http://www.w3.org/2003/06/sw-vocab-status/ns#term_status> "testing" .


###  http://xmlns.com/foaf/0.1/homepage
<http://xmlns.com/foaf/0.1/homepage> rdf:type owl:ObjectProperty ;
                                     rdfs:subPropertyOf <http://xmlns.com/foaf/0.1/isPrimaryTopicOf> ,
                                                        <http://xmlns.com/foaf/0.1/page> ;
                                     rdf:type owl:InverseFunctionalProperty ;
                                     rdfs:domain owl:Thing ;
                                     rdfs:range <http://xmlns.com/foaf/0.1/Document> ;
                                     rdfs:comment "A homepage for some thing." ;
                                     rdfs:isDefinedBy <http://xmlns.com/foaf/0.1/> ;
                                     rdfs:label "homepage" ;
                                     <http://www.w3.org/2003/06/sw-vocab-status/ns#term_status> "stable" .


###  http://xmlns.com/foaf/0.1/isPrimaryTopicOf
<http://xmlns.com/foaf/0.1/isPrimaryTopicOf> rdf:type owl:ObjectProperty ;
                                             rdfs:subPropertyOf <http://xmlns.com/foaf/0.1/page> ;
                                             owl:inverseOf <http://xmlns.com/foaf/0.1/primaryTopic> ;
                                             rdf:type owl:InverseFunctionalProperty ;
                                             rdfs:domain owl:Thing ;
                                             rdfs:range <http://xmlns.com/foaf/0.1/Document> ;
                                             rdfs:comment "A document that this thing is the primary topic of." ;
                                             rdfs:isDefinedBy <http://xmlns.com/foaf/0.1/> ;
                                             rdfs:label "is primary topic of" ;
                                             <http://www.w3.org/2003/06/sw-vocab-status/ns#term_status> "stable" .


###  http://xmlns.com/foaf/0.1/knows
<http://xmlns.com/foaf/0.1/knows> rdf:type owl:ObjectProperty ;
                                  rdfs:comment "A person known by this person (indicating some level of reciprocated interaction between the parties)." ;
                                  rdfs:isDefinedBy <http://xmlns.com/foaf/0.1/> ;
                                  rdfs:label "knows" ;
                                  <http://www.w3.org/2003/06/sw-vocab-status/ns#term_status> "stable" .


###  http://xmlns.com/foaf/0.1/openid
<http://xmlns.com/foaf/0.1/openid> rdf:type owl:ObjectProperty ;
                                   rdfs:subPropertyOf <http://xmlns.com/foaf/0.1/isPrimaryTopicOf> ;
                                   rdf:type owl:InverseFunctionalProperty ;
                                   rdfs:domain <http://xmlns.com/foaf/0.1/Agent> ;
                                   rdfs:range <http://xmlns.com/foaf/0.1/Document> ;
                                   rdfs:comment "An OpenID for an Agent." ;
                                   rdfs:isDefinedBy <http://xmlns.com/foaf/0.1/> ;
                                   rdfs:label "openid" ;
                                   <http://www.w3.org/2003/06/sw-vocab-status/ns#term_status> "testing" .


###  http://xmlns.com/foaf/0.1/page
<http://xmlns.com/foaf/0.1/page> rdf:type owl:ObjectProperty ;
                                 owl:inverseOf <http://xmlns.com/foaf/0.1/topic> ;
                                 rdfs:domain owl:Thing ;
                                 rdfs:range <http://xmlns.com/foaf/0.1/Document> ;
                                 rdfs:comment "A page or document about this thing." ;
                                 rdfs:isDefinedBy <http://xmlns.com/foaf/0.1/> ;
                                 rdfs:label "page" ;
                                 <http://www.w3.org/2003/06/sw-vocab-status/ns#term_status> "stable" .


###  http://xmlns.com/foaf/0.1/primaryTopic
<http://xmlns.com/foaf/0.1/primaryTopic> rdf:type owl:ObjectProperty ,
                                                  owl:FunctionalProperty ;
                                         rdfs:domain <http://xmlns.com/foaf/0.1/Document> ;
                                         rdfs:range owl:Thing ;
                                         rdfs:comment "The primary topic of some page or document." ;
                                         rdfs:isDefinedBy <http://xmlns.com/foaf/0.1/> ;
                                         rdfs:label "primary topic" ;
                                         <http://www.w3.org/2003/06/sw-vocab-status/ns#term_status> "stable" .


###  http://xmlns.com/foaf/0.1/publications
<http://xmlns.com/foaf/0.1/publications> rdf:type owl:ObjectProperty ;
                                         rdfs:range <http://xmlns.com/foaf/0.1/Document> ;
                                         rdfs:comment "A link to the publications of this person." ;
                                         rdfs:isDefinedBy <http://xmlns.com/foaf/0.1/> ;
                                         rdfs:label "publications" ;
                                         <http://www.w3.org/2003/06/sw-vocab-status/ns#term_status> "testing" .


###  http://xmlns.com/foaf/0.1/schoolHomepage
<http://xmlns.com/foaf/0.1/schoolHomepage> rdf:type owl:ObjectProperty ;
                                           rdfs:range <http://xmlns.com/foaf/0.1/Document> ;
                                           rdfs:comment "A homepage of a school attended by the person." ;
                                           rdfs:isDefinedBy <http://xmlns.com/foaf/0.1/> ;
                                           rdfs:label "schoolHomepage" ;
                                           <http://www.w3.org/2003/06/sw-vocab-status/ns#term_status> "testing" .


###  http://xmlns.com/foaf/0.1/topic
<http://xmlns.com/foaf/0.1/topic> rdf:type owl:ObjectProperty ;
                                  rdfs:domain <http://xmlns.com/foaf/0.1/Document> ;
                                  rdfs:range owl:Thing ;
                                  rdfs:comment "A topic of some page or document." ;
                                  rdfs:isDefinedBy <http://xmlns.com/foaf/0.1/> ;
                                  rdfs:label "topic" ;
                                  <http://www.w3.org/2003/06/sw-vocab-status/ns#term_status> "testing" .


###  http://xmlns.com/foaf/0.1/topic_interest
<http://xmlns.com/foaf/0.1/topic_interest> rdf:type owl:ObjectProperty ;
                                           rdfs:domain <http://xmlns.com/foaf/0.1/Agent> ;
                                           rdfs:range owl:Thing ;
                                           rdfs:comment "A thing of interest to this person." ;
                                           rdfs:isDefinedBy <http://xmlns.com/foaf/0.1/> ;
                                           rdfs:label "topic_interest" ;
                                           <http://www.w3.org/2003/06/sw-vocab-status/ns#term_status> "testing" .


###  https://schema.org/about
<https://schema.org/about> rdf:type owl:ObjectProperty ;
                           rdfs:domain <https://schema.org/CreativeWork> ;
                           rdfs:comment "The subject matter of the content." ;
                           rdfs:label "about" ;
                           <https://schema.org/inverseOf> <https://schema.org/subjectOf> ;
                           <https://schema.org/source> <https://github.com/schemaorg/schemaorg/issues/1670> .


###  https://schema.org/accountablePerson
<https://schema.org/accountablePerson> rdf:type owl:ObjectProperty ;
                                       rdfs:domain <https://schema.org/CreativeWork> ;
                                       rdfs:range <https://schema.org/Person> ;
                                       rdfs:comment "Specifies the Person that is legally accountable for the CreativeWork." ;
                                       rdfs:label "accountablePerson" .


###  https://schema.org/audience
<https://schema.org/audience> rdf:type owl:ObjectProperty ;
                              rdfs:domain <https://schema.org/CreativeWork> ;
                              rdfs:comment "An intended audience, i.e. a group for whom something was created." ;
                              rdfs:label "audience" .


###  https://schema.org/author
<https://schema.org/author> rdf:type owl:ObjectProperty ;
                            rdfs:domain <https://schema.org/CreativeWork> ;
                            rdfs:range <https://schema.org/Organization> ,
                                       <https://schema.org/Person> ;
                            rdfs:comment "The author of this content or rating. Please note that author is special in that HTML 5 provides a special mechanism for indicating authorship via the rel tag. That is equivalent to this and may be used interchangeably." ;
                            rdfs:label "author" .


###  https://schema.org/character
<https://schema.org/character> rdf:type owl:ObjectProperty ;
                               rdfs:domain <https://schema.org/CreativeWork> ;
                               rdfs:range <https://schema.org/Person> ;
                               rdfs:comment "Fictional person connected with a creative work." ;
                               rdfs:label "character" .


###  https://schema.org/citation
<https://schema.org/citation> rdf:type owl:ObjectProperty ;
                              rdfs:domain <https://schema.org/CreativeWork> ;
                              rdfs:range <https://schema.org/CreativeWork> ;
                              rdfs:comment "A citation or reference to another creative work, such as another publication, web page, scholarly article, etc." ;
                              rdfs:label "citation" .


###  https://schema.org/contentLocation
<https://schema.org/contentLocation> rdf:type owl:ObjectProperty ;
                                     rdfs:domain <https://schema.org/CreativeWork> ;
                                     rdfs:comment "The location depicted or described in the content. For example, the location in a photograph or painting." ;
                                     rdfs:label "contentLocation" .


###  https://schema.org/contributor
<https://schema.org/contributor> rdf:type owl:ObjectProperty ;
                                 rdfs:domain <https://schema.org/CreativeWork> ;
                                 rdfs:range <https://schema.org/Organization> ,
                                            <https://schema.org/Person> ;
                                 rdfs:comment "A secondary contributor to the CreativeWork or Event." ;
                                 rdfs:label "contributor" .


###  https://schema.org/creator
<https://schema.org/creator> rdf:type owl:ObjectProperty ;
                             rdfs:domain <https://schema.org/CreativeWork> ;
                             rdfs:range <https://schema.org/Organization> ,
                                        <https://schema.org/Person> ;
                             rdfs:comment "The creator/author of this CreativeWork. This is the same as the Author property for CreativeWork." ;
                             rdfs:label "creator" .


###  https://schema.org/dateCreated
<https://schema.org/dateCreated> rdf:type owl:ObjectProperty ;
                                 rdfs:domain <https://schema.org/CreativeWork> ;
                                 rdfs:range <https://schema.org/Date> ,
                                            <https://schema.org/DateTime> ;
                                 rdfs:comment "The date on which the CreativeWork was created or the item was added to a DataFeed." ;
                                 rdfs:label "dateCreated" .


###  https://schema.org/datePublished
<https://schema.org/datePublished> rdf:type owl:ObjectProperty ;
                                   rdfs:domain <https://schema.org/CreativeWork> ;
                                   rdfs:range <https://schema.org/Date> ,
                                              <https://schema.org/DateTime> ;
                                   rdfs:comment "Date of first broadcast/publication." ;
                                   rdfs:label "datePublished" .


###  https://schema.org/inLanguage
<https://schema.org/inLanguage> rdf:type owl:ObjectProperty ;
                                rdfs:domain <https://schema.org/CreativeWork> ;
                                rdfs:range <https://schema.org/Language> ;
                                rdfs:comment "The language of the content or performance or used in an action. Please use one of the language codes from the [IETF BCP 47 standard](http://tools.ietf.org/html/bcp47). See also [[availableLanguage]]." ;
                                rdfs:label "inLanguage" .


###  https://schema.org/keywords
<https://schema.org/keywords> rdf:type owl:ObjectProperty ;
                              rdfs:domain <https://schema.org/CreativeWork> ;
                              rdfs:range <https://schema.org/DefinedTerm> ;
                              rdfs:comment "Keywords or tags used to describe this content. Multiple entries in a keywords list are typically delimited by commas." ;
                              rdfs:label "keywords" .


###  https://schema.org/mainEntity
<https://schema.org/mainEntity> rdf:type owl:ObjectProperty ;
                                rdfs:subPropertyOf <https://schema.org/about> ;
                                rdfs:domain <https://schema.org/CreativeWork> ;
                                rdfs:comment "Indicates the primary entity described in some page or other CreativeWork." ;
                                rdfs:label "mainEntity" ;
                                <https://schema.org/inverseOf> <https://schema.org/mainEntityOfPage> .


###  https://schema.org/spatialCoverage
<https://schema.org/spatialCoverage> rdf:type owl:ObjectProperty ;
                                     rdfs:subPropertyOf <https://schema.org/contentLocation> ;
                                     rdfs:domain <https://schema.org/CreativeWork> ;
                                     rdfs:comment """The spatialCoverage of a CreativeWork indicates the place(s) which are the focus of the content. It is a subproperty of
      contentLocation intended primarily for more technical and detailed materials. For example with a Dataset, it indicates
      areas that the dataset describes: a dataset of New York weather would have spatialCoverage which was the place: the state of New York.""" ;
                                     rdfs:label "spatialCoverage" .


###  https://w3id.org/skgo/modsci#doingStudies
<https://w3id.org/skgo/modsci#doingStudies> rdf:type owl:ObjectProperty ;
                                            rdfs:domain <https://w3id.org/skgo/modsci#Scientist> ;
                                            rdfs:range <https://w3id.org/skgo/modsci#ModernScience> .


###  https://w3id.org/skgo/modsci#hasCloseRelationshipTo
<https://w3id.org/skgo/modsci#hasCloseRelationshipTo> rdf:type owl:ObjectProperty ,
                                                               owl:SymmetricProperty ,
                                                               owl:ReflexiveProperty ;
                                                      rdfs:domain <https://w3id.org/skgo/modsci#ModernScience> ;
                                                      rdfs:range <https://w3id.org/skgo/modsci#ModernScience> .


###  https://w3id.org/skgo/modsci#inspiredFrom
<https://w3id.org/skgo/modsci#inspiredFrom> rdf:type owl:ObjectProperty ,
                                                     owl:FunctionalProperty ;
                                            rdfs:domain <https://w3id.org/skgo/modsci#ScientificMethod> ;
                                            rdfs:range [ rdf:type owl:Class ;
                                                         owl:unionOf ( <http://sweetontology.net/phen/Phenomenon>
                                                                       <https://w3id.org/skgo/modsci#ScientificDiscovery>
                                                                     )
                                                       ] .


###  https://w3id.org/skgo/modsci#inspiredFromPhenomenon
<https://w3id.org/skgo/modsci#inspiredFromPhenomenon> rdf:type owl:ObjectProperty ;
                                                      rdfs:subPropertyOf <https://w3id.org/skgo/modsci#inspiredFrom> .


###  https://w3id.org/skgo/modsci#inspiredFromScientificDiscovery
<https://w3id.org/skgo/modsci#inspiredFromScientificDiscovery> rdf:type owl:ObjectProperty ;
                                                               rdfs:subPropertyOf <https://w3id.org/skgo/modsci#inspiredFrom> .


###  https://w3id.org/skgo/modsci#requiresKnowledgeFrom
<https://w3id.org/skgo/modsci#requiresKnowledgeFrom> rdf:type owl:ObjectProperty ,
                                                              owl:ReflexiveProperty ;
                                                     rdfs:domain <https://w3id.org/skgo/modsci#ModernScience> ;
                                                     rdfs:range <https://w3id.org/skgo/modsci#ModernScience> .


###  https://w3id.org/skgo/modsci#scientistBelongsTo
<https://w3id.org/skgo/modsci#scientistBelongsTo> rdf:type owl:ObjectProperty ;
                                                  rdfs:domain <https://w3id.org/skgo/modsci#Scientist> ;
                                                  rdfs:range <https://w3id.org/skgo/modsci#ModernScience> .


#################################################################
#    Data properties
#################################################################

###  http://www.is-unit4.org/ontology/EducationalMaterials#hasAge
:hasAge rdf:type owl:DatatypeProperty ;
        rdfs:domain <https://schema.org/Person> ;
        rdfs:range xsd:int ;
        rdfs:comment "The age of an student or, more generaly, of a person"@en ;
        rdfs:label "Has age"@en .


###  http://xmlns.com/foaf/0.1/givenName
<http://xmlns.com/foaf/0.1/givenName> rdf:type owl:DatatypeProperty ;
                                      rdfs:comment "The given name of some person." ;
                                      rdfs:isDefinedBy <http://xmlns.com/foaf/0.1/> ;
                                      rdfs:label "Given name" ;
                                      <http://www.w3.org/2003/06/sw-vocab-status/ns#term_status> "testing" .


###  http://xmlns.com/foaf/0.1/title
<http://xmlns.com/foaf/0.1/title> rdf:type owl:DatatypeProperty ;
                                  rdfs:comment "Title (Mr, Mrs, Ms, Dr. etc)" ;
                                  rdfs:isDefinedBy <http://xmlns.com/foaf/0.1/> ;
                                  rdfs:label "title" ;
                                  <http://www.w3.org/2003/06/sw-vocab-status/ns#term_status> "testing" .


#################################################################
#    Classes
#################################################################

###  http://linkedscience.org/teach/ns#Assignment
<http://linkedscience.org/teach/ns#Assignment> rdf:type owl:Class ;
                                               rdfs:subClassOf :Evaluation ;
                                               rdfs:comment """Assignment of a course, for example an exercise.
"""@en ;
                                               rdfs:isDefinedBy <http://linkedscience.org/teach/ns> ;
                                               rdfs:label "Assignment"@en .


###  http://linkedscience.org/teach/ns#Lecture
<http://linkedscience.org/teach/ns#Lecture> rdf:type owl:Class ;
                                            rdfs:comment """Lecture of the course.
"""@en ;
                                            rdfs:isDefinedBy <http://linkedscience.org/teach/ns> ;
                                            rdfs:label "Lecture"@en .


###  http://linkedscience.org/teach/ns#Module
<http://linkedscience.org/teach/ns#Module> rdf:type owl:Class ;
                                           rdfs:comment """Module (i.e. a set of courses) which the course belongs to.
"""@en ;
                                           rdfs:isDefinedBy <http://linkedscience.org/teach/ns> ;
                                           rdfs:label "Module"@en .


###  http://linkedscience.org/teach/ns#Student
<http://linkedscience.org/teach/ns#Student> rdf:type owl:Class ;
                                            rdfs:comment """Student of the course.
"""@en ;
                                            rdfs:isDefinedBy <http://linkedscience.org/teach/ns> ;
                                            rdfs:label "Student"@en .


###  http://linkedscience.org/teach/ns#StudentGroup
<http://linkedscience.org/teach/ns#StudentGroup> rdf:type owl:Class ;
                                                 rdfs:comment """StudentGroup of the course.
"""@en ;
                                                 rdfs:isDefinedBy <http://linkedscience.org/teach/ns> ;
                                                 rdfs:label "StudentGroup"@en .


###  http://linkedscience.org/teach/ns#StudyProgram
<http://linkedscience.org/teach/ns#StudyProgram> rdf:type owl:Class ;
                                                 rdfs:comment """StudyProgram which the course is part of.
"""@en ;
                                                 rdfs:isDefinedBy <http://linkedscience.org/teach/ns> ;
                                                 rdfs:label "StudyProgram"@en .


###  http://linkedscience.org/teach/ns#Teacher
<http://linkedscience.org/teach/ns#Teacher> rdf:type owl:Class ;
                                            rdfs:comment """Teacher of the course.
"""@en ;
                                            rdfs:isDefinedBy <http://linkedscience.org/teach/ns> ;
                                            rdfs:label "Teacher"@en .


###  http://ns.inria.fr/semed/eduprogression/v1#Course
<http://ns.inria.fr/semed/eduprogression/v1#Course> rdf:type owl:Class ;
                                                    rdfs:comment "In the French educational system, skills that students are expected to develop, are defined by cycle and each cycle is organized into course."@en ;
                                                    rdfs:isDefinedBy <http://ns.inria.fr/semed/eduprogression#> ;
                                                    rdfs:label "Cours"@fr ,
                                                               "Course "@en ;
                                                    <http://www.w3.org/2003/06/sw-vocab-status/ns#term_status> "stable" .


###  http://ns.inria.fr/semed/eduprogression/v1#EKS
<http://ns.inria.fr/semed/eduprogression/v1#EKS> rdf:type owl:Class ;
                                                 rdfs:comment "An element of knowledge and skills is an instance of this class and it is associated to a set of knowledge pieces (class Knowledge) and skills (class Skill) for a specific French school cycle (class Course) containing reference points (class PointOfReference) and also a vocabulary of associated terms (class Vocabulary)."@en ;
                                                 rdfs:isDefinedBy <http://ns.inria.fr/semed/eduprogression#> ;
                                                 rdfs:label "Element de connaissances et de competences"@fr ,
                                                            "Element of knowledge and skills "@en ;
                                                 <http://www.w3.org/2003/06/sw-vocab-status/ns#term_status> "stable" .


###  http://ns.inria.fr/semed/eduprogression/v1#Knowledge
<http://ns.inria.fr/semed/eduprogression/v1#Knowledge> rdf:type owl:Class ;
                                                       rdfs:comment "It is represented by class Knowledge and each of its instances is a skos:Concept that is part of a skos:ConceptScheme that contains all the knowledge pieces of a given progression. An instance of EKS is related to an instance of Knowledge through property hasKnowledge."@en ;
                                                       rdfs:isDefinedBy <http://ns.inria.fr/semed/eduprogression#> ;
                                                       rdfs:label "Connaissance"@fr ,
                                                                  "Knowledge "@en ;
                                                       <http://www.w3.org/2003/06/sw-vocab-status/ns#term_status> "stable" .


###  http://ns.inria.fr/semed/eduprogression/v1#LearningDomain
<http://ns.inria.fr/semed/eduprogression/v1#LearningDomain> rdf:type owl:Class ;
                                                            rdfs:comment "A learning domain is represented by an instance of the LearningDomain class, and it is also an instance of skos:Concept that is part of (only) one skos:ConceptScheme containing the only learning domains of a progression. Also, as they are SKOS concepts, learning domains are hierarchically structured by using the skos:broader and/or skos:narrower properties. A learning domain can be associated to a Progression or to an EKS."@en ;
                                                            rdfs:isDefinedBy <http://ns.inria.fr/semed/eduprogression#> ;
                                                            rdfs:label "Domaine d'enseignement"@fr ,
                                                                       "Learning domain"@en ;
                                                            <http://www.w3.org/2003/06/sw-vocab-status/ns#term_status> "stable" .


###  http://ns.inria.fr/semed/eduprogression/v1#PointOfReference
<http://ns.inria.fr/semed/eduprogression/v1#PointOfReference> rdf:type owl:Class ;
                                                              rdfs:comment "An instance of class PointOfReference represents an educational reference element on a specific element of knowledge and skills (an instance of EKS). An instance of EKS is related to an instance of class PointOfReference through the property hasPointOfReference."@en ;
                                                              rdfs:isDefinedBy <http://ns.inria.fr/semed/eduprogression#> ;
                                                              rdfs:label "Point of reference"@en ,
                                                                         "Repère"@fr ;
                                                              <http://www.w3.org/2003/06/sw-vocab-status/ns#term_status> "stable" .


###  http://ns.inria.fr/semed/eduprogression/v1#Progression
<http://ns.inria.fr/semed/eduprogression/v1#Progression> rdf:type owl:Class ;
                                                         rdfs:comment "A progression is represented by an instance of class Progression. It can be further described by using the Dublin Core or RDFS vocabularies. A progression can be associated to an existing learning domain (through the hasLearningDomain property) and to one or several EKSs (through the hasEKS property)."@en ;
                                                         rdfs:isDefinedBy <http://ns.inria.fr/semed/eduprogression#> ;
                                                         rdfs:label "Progression"@en ,
                                                                    "Progression"@fr ;
                                                         <http://www.w3.org/2003/06/sw-vocab-status/ns#term_status> "stable" .


###  http://ns.inria.fr/semed/eduprogression/v1#Skill
<http://ns.inria.fr/semed/eduprogression/v1#Skill> rdf:type owl:Class ;
                                                   rdfs:comment "It is represented by class Skill and described as well by using the Dublin Core and RDFS vocabularies. An instance of EKS is related to an instance of Skill through property hasSkill."@en ;
                                                   rdfs:isDefinedBy <http://ns.inria.fr/semed/eduprogression#> ;
                                                   rdfs:label "Competence"@fr ,
                                                              "Skill"@en ;
                                                   <http://www.w3.org/2003/06/sw-vocab-status/ns#term_status> "stable" .


###  http://purl.org/dc/dcmitype/Image
<http://purl.org/dc/dcmitype/Image> rdf:type owl:Class ;
                                    owl:equivalentClass <https://schema.org/ImageObject> .


###  http://sweetontology.net/phen/Phenomenon
<http://sweetontology.net/phen/Phenomenon> rdf:type owl:Class .


###  http://www.is-unit4.org/ontology/EducationalMaterials#AlphabeticGrade
:AlphabeticGrade rdf:type owl:Class ;
                 rdfs:subClassOf :GradingSystem ;
                 rdfs:comment "Marks from A to F"@en ;
                 rdfs:label "Alphabetic Grading System"@en .


###  http://www.is-unit4.org/ontology/EducationalMaterials#ArtsAndHumanities
:ArtsAndHumanities rdf:type owl:Class ;
                   rdfs:subClassOf <http://ns.inria.fr/semed/eduprogression/v1#LearningDomain> ;
                   rdfs:comment "Philosophy and arts field"@en ;
                   rdfs:label "Arts and humanities"@en .


###  http://www.is-unit4.org/ontology/EducationalMaterials#AtmosphericalMap
:AtmosphericalMap rdf:type owl:Class ;
                  rdfs:subClassOf :GeographicMap ;
                  rdfs:comment "Includes all kinds of maps containing atmospherical variables information"@en ;
                  rdfs:label "Atmospherical map"@en .


###  http://www.is-unit4.org/ontology/EducationalMaterials#ClosedLicenses
:ClosedLicenses rdf:type owl:Class ;
                rdfs:subClassOf :License ;
                rdfs:comment "Licenses were the author somehow restriicts the use of the product"@en ;
                rdfs:label "Closed licenses"@en .


###  http://www.is-unit4.org/ontology/EducationalMaterials#Dictionary
:Dictionary rdf:type owl:Class ;
            rdfs:subClassOf :ReferenceBook ;
            rdfs:comment "A dictionary of any kind"@en ;
            rdfs:label "Dictionary"@en .


###  http://www.is-unit4.org/ontology/EducationalMaterials#Evaluation
:Evaluation rdf:type owl:Class ;
            rdfs:comment "Evaluation method selected" ;
            rdfs:label "Evaluation" .


###  http://www.is-unit4.org/ontology/EducationalMaterials#Exam
:Exam rdf:type owl:Class ;
      rdfs:subClassOf :Evaluation ;
      rdfs:comment "Scheduled and evaluated that last short time periods"@en ;
      rdfs:label "Exam"@en .


###  http://www.is-unit4.org/ontology/EducationalMaterials#Exercise
:Exercise rdf:type owl:Class ;
          rdfs:subClassOf <http://linkedscience.org/teach/ns#Assignment> ;
          rdfs:comment "Academic exercise that needs to be handled and evaluated"@en ;
          rdfs:label "Exercise"@en .


###  http://www.is-unit4.org/ontology/EducationalMaterials#GeographicMap
:GeographicMap rdf:type owl:Class ;
               rdfs:subClassOf <https://schema.org/Map> ;
               rdfs:comment "General class that includes all kinds of non-political maps"@en ;
               rdfs:label "Geographic Map"@en .


###  http://www.is-unit4.org/ontology/EducationalMaterials#GradingSystem
:GradingSystem rdf:type owl:Class ;
               rdfs:comment "A specific standard way to present students marks"@en ;
               rdfs:label "Grading System"@en .


###  http://www.is-unit4.org/ontology/EducationalMaterials#HydrographicMap
:HydrographicMap rdf:type owl:Class ;
                 rdfs:subClassOf :GeographicMap ;
                 rdfs:comment "Map that includes rivers seas and all other natural and artificial elements related with them"@en ;
                 rdfs:label "Hydrographic map"@en .


###  http://www.is-unit4.org/ontology/EducationalMaterials#License
:License rdf:type owl:Class ;
         rdfs:comment "A license to protect all kind of creative works and, specifically, educational materials"@en ;
         rdfs:label "License"@en .


###  http://www.is-unit4.org/ontology/EducationalMaterials#LiteratureBook
:LiteratureBook rdf:type owl:Class ;
                rdfs:subClassOf <https://schema.org/Book> ;
                rdfs:comment "Books created with an artistic intention"@en ;
                rdfs:label "Literature Book"@en .


###  http://www.is-unit4.org/ontology/EducationalMaterials#NaturalSciencesDomain
:NaturalSciencesDomain rdf:type owl:Class ;
                       rdfs:subClassOf <http://ns.inria.fr/semed/eduprogression/v1#LearningDomain> ;
                       rdfs:comment "Physical and biological sciences field"@en ;
                       rdfs:label "Natural Sciences Domain"@en .


###  http://www.is-unit4.org/ontology/EducationalMaterials#NominalGrade
:NominalGrade rdf:type owl:Class ;
              rdfs:subClassOf :GradingSystem ;
              rdfs:comment "Qualitative system that includes categories form failed to outstanding"@en ;
              rdfs:label "Nominal Grading System"@en .


###  http://www.is-unit4.org/ontology/EducationalMaterials#NovelBook
:NovelBook rdf:type owl:Class ;
           rdfs:subClassOf :LiteratureBook ;
           rdfs:comment "A novel"@en ;
           rdfs:label "Novel Book"@en .


###  http://www.is-unit4.org/ontology/EducationalMaterials#NumericGrade
:NumericGrade rdf:type owl:Class ;
              rdfs:subClassOf :GradingSystem ;
              rdfs:comment "Marks form 0 to 10 or from 0 to 100"@en ;
              rdfs:label "Numeric Grading System"@en .


###  http://www.is-unit4.org/ontology/EducationalMaterials#OpenLicenses
:OpenLicenses rdf:type owl:Class ;
              rdfs:subClassOf :License ;
              rdfs:comment "Licenses were the use of the product is free except to commercialize it (sometimes)"@en ;
              rdfs:label "Open licenses"@en .


###  http://www.is-unit4.org/ontology/EducationalMaterials#PoetryBook
:PoetryBook rdf:type owl:Class ;
            rdfs:subClassOf :LiteratureBook ;
            rdfs:comment "A book of poems"@en ;
            rdfs:label "Poetry Book"@en .


###  http://www.is-unit4.org/ontology/EducationalMaterials#PoliticalMap
:PoliticalMap rdf:type owl:Class ;
              rdfs:subClassOf <https://schema.org/Map> ;
              rdfs:comment "Map conaining frontiers and other artificial elements"@en ;
              rdfs:label "Political Map"@en .


###  http://www.is-unit4.org/ontology/EducationalMaterials#PracticalApplication
:PracticalApplication rdf:type owl:Class ;
                      rdfs:subClassOf <http://linkedscience.org/teach/ns#Assignment> ;
                      rdfs:comment "More extensive assignment that is evaluated in the context of a course"@en ;
                      rdfs:label "Practical Application"@en .


###  http://www.is-unit4.org/ontology/EducationalMaterials#ReferenceBook
:ReferenceBook rdf:type owl:Class ;
               rdfs:subClassOf <https://schema.org/Book> ;
               rdfs:comment "Books to consult information"@en ;
               rdfs:label "Reference Book"@en .


###  http://www.is-unit4.org/ontology/EducationalMaterials#SocialSciencesDomain
:SocialSciencesDomain rdf:type owl:Class ;
                      rdfs:subClassOf <http://ns.inria.fr/semed/eduprogression/v1#LearningDomain> ;
                      rdfs:comment "Antoropological and historical scieces field"@en ;
                      rdfs:label "Social sciences domain"@en .


###  http://www.is-unit4.org/ontology/EducationalMaterials#TextBook
:TextBook rdf:type owl:Class ;
          rdfs:subClassOf <https://schema.org/Book> ;
          rdfs:comment "Academic or theoretical books"@en ;
          rdfs:label "Text Book"@en .


###  http://www.is-unit4.org/ontology/EducationalMaterials#TheaterBook
:TheaterBook rdf:type owl:Class ;
             rdfs:subClassOf :LiteratureBook ;
             rdfs:comment "A written play"@en ;
             rdfs:label "Theater Book"@en .


###  http://www.is-unit4.org/ontology/EducationalMaterials#TopographicMap
:TopographicMap rdf:type owl:Class ;
                rdfs:subClassOf :GeographicMap ;
                rdfs:comment "Map that may include all kind of geological formations"@en ;
                rdfs:label "Topographic Map"@en .


###  http://www.is-unit4.org/ontology/EducationalMaterials#WebArticle
:WebArticle rdf:type owl:Class ;
            rdfs:subClassOf <https://schema.org/Article> ;
            rdfs:comment "An article fully available in a web page"@en ;
            rdfs:label "Web article"@en .


###  http://www.w3.org/2002/07/owl#Thing
owl:Thing rdfs:label "Thing" .


###  http://www.w3.org/2004/02/skos/core#Concept
<http://www.w3.org/2004/02/skos/core#Concept> rdf:type owl:Class .


###  http://www.w3.org/2004/02/skos/core#ConceptScheme
<http://www.w3.org/2004/02/skos/core#ConceptScheme> rdf:type owl:Class .


###  http://xmlns.com/foaf/0.1/Agent
<http://xmlns.com/foaf/0.1/Agent> rdf:type owl:Class .


###  http://xmlns.com/foaf/0.1/Document
<http://xmlns.com/foaf/0.1/Document> rdf:type owl:Class ;
                                     owl:disjointWith <http://xmlns.com/foaf/0.1/Project> ;
                                     rdfs:comment "A document." ;
                                     rdfs:isDefinedBy <http://xmlns.com/foaf/0.1/> ;
                                     rdfs:label "Document" ;
                                     <http://www.w3.org/2003/06/sw-vocab-status/ns#term_status> "stable" .


###  http://xmlns.com/foaf/0.1/Group
<http://xmlns.com/foaf/0.1/Group> rdf:type owl:Class .


###  http://xmlns.com/foaf/0.1/Image
<http://xmlns.com/foaf/0.1/Image> rdf:type owl:Class ;
                                  rdfs:subClassOf <http://xmlns.com/foaf/0.1/Document> ;
                                  rdfs:comment "An image." ;
                                  rdfs:isDefinedBy <http://xmlns.com/foaf/0.1/> ;
                                  rdfs:label "Image" ;
                                  <http://www.w3.org/2003/06/sw-vocab-status/ns#term_status> "stable" .


###  http://xmlns.com/foaf/0.1/PersonalProfileDocument
<http://xmlns.com/foaf/0.1/PersonalProfileDocument> rdf:type owl:Class ;
                                                    rdfs:subClassOf <http://xmlns.com/foaf/0.1/Document> ;
                                                    rdfs:comment "A personal profile RDF document." ;
                                                    rdfs:label "PersonalProfileDocument" ;
                                                    <http://www.w3.org/2003/06/sw-vocab-status/ns#term_status> "testing" .


###  http://xmlns.com/foaf/0.1/Project
<http://xmlns.com/foaf/0.1/Project> rdf:type owl:Class .


###  https://schema.org/APIReference
<https://schema.org/APIReference> rdf:type owl:Class ;
                                  rdfs:subClassOf <https://schema.org/TechArticle> ;
                                  rdfs:comment "Reference documentation for application programming interfaces (APIs)." ;
                                  rdfs:label "APIReference" .


###  https://schema.org/Article
<https://schema.org/Article> rdf:type owl:Class ;
                             rdfs:subClassOf <https://schema.org/CreativeWork> ;
                             rdfs:comment "An article, such as a news article or piece of investigative report. Newspapers and magazines have articles of many different types and this is intended to cover them all.\\n\\nSee also [blog post](http://blog.schema.org/2014/09/schemaorg-support-for-bibliographic_2.html)." ;
                             rdfs:label "Article" ;
                             <https://schema.org/source> <http://www.w3.org/wiki/WebSchemas/SchemaDotOrgSources#source_rNews> .


###  https://schema.org/AudioObject
<https://schema.org/AudioObject> rdf:type owl:Class ;
                                 rdfs:subClassOf <https://schema.org/MediaObject> ;
                                 rdfs:comment "An audio file." ;
                                 rdfs:label "AudioObject" ;
                                 <https://schema.org/source> <http://www.w3.org/wiki/WebSchemas/SchemaDotOrgSources#source_rNews> .


###  https://schema.org/Blog
<https://schema.org/Blog> rdf:type owl:Class ;
                          rdfs:subClassOf <https://schema.org/CreativeWork> ;
                          rdfs:comment "A [blog](https://en.wikipedia.org/wiki/Blog), sometimes known as a \"weblog\". Note that the individual posts ([[BlogPosting]]s) in a [[Blog]] are often colloqually referred to by the same term." ;
                          rdfs:label "Blog" .


###  https://schema.org/Book
<https://schema.org/Book> rdf:type owl:Class ;
                          rdfs:subClassOf <https://schema.org/CreativeWork> ;
                          rdfs:comment "A book." ;
                          rdfs:label "Book"@en .


###  https://schema.org/Code
<https://schema.org/Code> rdf:type owl:Class ;
                          rdfs:subClassOf <https://schema.org/CreativeWork> ;
                          rdfs:comment "Computer programming source code. Example: Full (compile ready) solutions, code snippet samples, scripts, templates." ;
                          rdfs:label "Code" .


###  https://schema.org/Course
<https://schema.org/Course> rdf:type owl:Class ;
                            rdfs:subClassOf <https://schema.org/CreativeWork> ;
                            rdfs:comment "A description of an educational course which may be offered as distinct instances at which take place at different times or take place at different locations, or be offered through different media or modes of study. An educational course is a sequence of one or more educational events and/or creative works which aims to build knowledge, competence or ability of learners." ;
                            rdfs:label "Course" .


###  https://schema.org/CreativeWork
<https://schema.org/CreativeWork> rdf:type owl:Class ;
                                  rdfs:comment "The most generic kind of creative work, including books, movies, photographs, software programs, etc." ;
                                  rdfs:label "CreativeWork" ;
                                  <https://schema.org/source> <http://www.w3.org/wiki/WebSchemas/SchemaDotOrgSources#source_rNews> .


###  https://schema.org/Date
<https://schema.org/Date> rdf:type owl:Class .


###  https://schema.org/DateTime
<https://schema.org/DateTime> rdf:type owl:Class .


###  https://schema.org/DefinedTerm
<https://schema.org/DefinedTerm> rdf:type owl:Class .


###  https://schema.org/DigitalDocument
<https://schema.org/DigitalDocument> rdf:type owl:Class ;
                                     rdfs:subClassOf <https://schema.org/CreativeWork> ;
                                     rdfs:comment "An electronic file or document." ;
                                     rdfs:label "DigitalDocument" .


###  https://schema.org/ImageObject
<https://schema.org/ImageObject> rdf:type owl:Class .


###  https://schema.org/Language
<https://schema.org/Language> rdf:type owl:Class .


###  https://schema.org/Map
<https://schema.org/Map> rdf:type owl:Class ;
                         rdfs:subClassOf <https://schema.org/CreativeWork> ;
                         rdfs:comment "A map." ;
                         rdfs:label "Map" .


###  https://schema.org/MediaObject
<https://schema.org/MediaObject> rdf:type owl:Class ;
                                 rdfs:subClassOf <https://schema.org/CreativeWork> ;
                                 rdfs:comment "A media object, such as an image, video, or audio object embedded in a web page or a downloadable dataset i.e. DataDownload. Note that a creative work may have many media objects associated with it on the same web page. For example, a page about a single song (MusicRecording) may have a music video (VideoObject), and a high and low bandwidth audio stream (2 AudioObject's)." ;
                                 rdfs:label "MediaObject" .


###  https://schema.org/NoteDigitalDocument
<https://schema.org/NoteDigitalDocument> rdf:type owl:Class ;
                                         rdfs:subClassOf <https://schema.org/DigitalDocument> ;
                                         rdfs:comment "A file containing a note, primarily for the author." ;
                                         rdfs:label "NoteDigitalDocument" .


###  https://schema.org/Organization
<https://schema.org/Organization> rdf:type owl:Class .


###  https://schema.org/Painting
<https://schema.org/Painting> rdf:type owl:Class ;
                              rdfs:subClassOf <https://schema.org/CreativeWork> ;
                              rdfs:comment "A painting." ;
                              rdfs:label "Painting" .


###  https://schema.org/Person
<https://schema.org/Person> rdf:type owl:Class .


###  https://schema.org/Photograph
<https://schema.org/Photograph> rdf:type owl:Class ;
                                rdfs:subClassOf <https://schema.org/CreativeWork> ;
                                rdfs:comment "A photograph." ;
                                rdfs:label "Photograph" .


###  https://schema.org/PresentationDigitalDocument
<https://schema.org/PresentationDigitalDocument> rdf:type owl:Class ;
                                                 rdfs:subClassOf <https://schema.org/DigitalDocument> ;
                                                 rdfs:comment "A file containing slides or used for a presentation." ;
                                                 rdfs:label "PresentationDigitalDocument" .


###  https://schema.org/PublicationVolume
<https://schema.org/PublicationVolume> rdf:type owl:Class ;
                                       rdfs:subClassOf <https://schema.org/CreativeWork> ;
                                       rdfs:comment "A part of a successively published publication such as a periodical or multi-volume work, often numbered. It may represent a time span, such as a year.\\n\\nSee also [blog post](http://blog.schema.org/2014/09/schemaorg-support-for-bibliographic_2.html)." ;
                                       rdfs:label "PublicationVolume" ;
                                       <https://schema.org/source> <http://www.w3.org/wiki/WebSchemas/SchemaDotOrgSources#source_bibex> .


###  https://schema.org/Report
<https://schema.org/Report> rdf:type owl:Class ;
                            rdfs:subClassOf <https://schema.org/Article> ;
                            rdfs:comment "A Report generated by governmental or non-governmental organization." ;
                            rdfs:label "Report" .


###  https://schema.org/ScholarlyArticle
<https://schema.org/ScholarlyArticle> rdf:type owl:Class ;
                                      rdfs:subClassOf <https://schema.org/Article> ;
                                      rdfs:comment "A scholarly article." ;
                                      rdfs:label "ScholarlyArticle" .


###  https://schema.org/SpreadsheetDigitalDocument
<https://schema.org/SpreadsheetDigitalDocument> rdf:type owl:Class ;
                                                rdfs:subClassOf <https://schema.org/DigitalDocument> ;
                                                rdfs:comment "A spreadsheet file." ;
                                                rdfs:label "SpreadsheetDigitalDocument" .


###  https://schema.org/TechArticle
<https://schema.org/TechArticle> rdf:type owl:Class ;
                                 rdfs:subClassOf <https://schema.org/Article> ;
                                 rdfs:comment "A technical article - Example: How-to (task) topics, step-by-step, procedural troubleshooting, specifications, etc." ;
                                 rdfs:label "TechArticle" .


###  https://schema.org/TextDigitalDocument
<https://schema.org/TextDigitalDocument> rdf:type owl:Class ;
                                         rdfs:subClassOf <https://schema.org/DigitalDocument> ;
                                         rdfs:comment "A file composed primarily of text." ;
                                         rdfs:label "TextDigitalDocument" .


###  https://schema.org/VideoObject
<https://schema.org/VideoObject> rdf:type owl:Class ;
                                 rdfs:subClassOf <https://schema.org/MediaObject> ;
                                 rdfs:comment "A video file." ;
                                 rdfs:label "VideoObject" ;
                                 <https://schema.org/source> <http://www.w3.org/wiki/WebSchemas/SchemaDotOrgSources#source_rNews> .


###  https://schema.org/VisualArtwork
<https://schema.org/VisualArtwork> rdf:type owl:Class ;
                                   rdfs:subClassOf <https://schema.org/CreativeWork> ;
                                   rdfs:comment "A work of art that is primarily visual in character." ;
                                   rdfs:label "VisualArtwork" ;
                                   <https://schema.org/source> <http://www.w3.org/wiki/WebSchemas/SchemaDotOrgSources#source_VisualArtworkClass> .


###  https://w3id.org/skgo/modsci#AcidbaseChemistry
<https://w3id.org/skgo/modsci#AcidbaseChemistry> rdf:type owl:Class ;
                                                 rdfs:subClassOf <https://w3id.org/skgo/modsci#Chemistry> ;
                                                 rdfs:comment "For chemicals that can behave as acids or bases" ;
                                                 rdfs:label "Acid–base Chemistry" .


###  https://w3id.org/skgo/modsci#Acoustics
<https://w3id.org/skgo/modsci#Acoustics> rdf:type owl:Class ;
                                         rdfs:subClassOf <https://w3id.org/skgo/modsci#AppliedSciences> ;
                                         rdfs:comment "Acoustics is a branch of continuum mechanics and is the study of sound, mechanical waves in gases, liquids, and solids." ;
                                         rdfs:label "Acoustics" .


###  https://w3id.org/skgo/modsci#Agriculture
<https://w3id.org/skgo/modsci#Agriculture> rdf:type owl:Class ;
                                           rdfs:subClassOf <https://w3id.org/skgo/modsci#AppliedSciences> ;
                                           rdfs:comment "Agriculture, also known as farming, is the process of producing food, feed, fiber and other desired products by cultivation of certain plants and the raising of domesticated animals." ;
                                           rdfs:label "Agriculture" .


###  https://w3id.org/skgo/modsci#AnalyticalChemistry
<https://w3id.org/skgo/modsci#AnalyticalChemistry> rdf:type owl:Class ;
                                                   rdfs:subClassOf <https://w3id.org/skgo/modsci#Chemistry> ;
                                                   rdfs:comment "Analytical chemistry is the analysis of material samples to gain an understanding of their chemical composition and structure." ;
                                                   rdfs:label "Analytical Chemistry" .


###  https://w3id.org/skgo/modsci#Anatomy
<https://w3id.org/skgo/modsci#Anatomy> rdf:type owl:Class ;
                                       rdfs:subClassOf <https://w3id.org/skgo/modsci#Biology> ;
                                       rdfs:comment "Anatomy is the study of the structure and organization of living things." ;
                                       rdfs:label "Anatomy" .


###  https://w3id.org/skgo/modsci#Anthropology
<https://w3id.org/skgo/modsci#Anthropology> rdf:type owl:Class ;
                                            rdfs:subClassOf <https://w3id.org/skgo/modsci#SocialSciences> ;
                                            rdfs:comment "Anthropology is the scientific study of humans, human behavior and societies in the past and present." ;
                                            rdfs:label "Anthropology" .


###  https://w3id.org/skgo/modsci#AppliedMathematics
<https://w3id.org/skgo/modsci#AppliedMathematics> rdf:type owl:Class ;
                                                  rdfs:subClassOf <https://w3id.org/skgo/modsci#AppliedSciences> ;
                                                  rdfs:comment "Applied mathematics is a branch of mathematics that concerns itself with the application of mathematical knowledge to other domains." ;
                                                  rdfs:label "Applied Mathematics" .


###  https://w3id.org/skgo/modsci#AppliedPhysics
<https://w3id.org/skgo/modsci#AppliedPhysics> rdf:type owl:Class ;
                                              rdfs:subClassOf <https://w3id.org/skgo/modsci#InterdisciplinaryStudies> ,
                                                              <https://w3id.org/skgo/modsci#Physics> ;
                                              rdfs:comment "Applied physics is intended for a particular technological or practical use." ;
                                              rdfs:label "Applied and Interdisciplinary Physics" .


###  https://w3id.org/skgo/modsci#AppliedSciences
<https://w3id.org/skgo/modsci#AppliedSciences> rdf:type owl:Class ;
                                               rdfs:subClassOf <https://w3id.org/skgo/modsci#ModernScience> ;
                                               rdfs:comment "Applied science is the use or the study of the use of scientific knowledge to develop technology." ;
                                               rdfs:label "Applied Sciences" .


###  https://w3id.org/skgo/modsci#Archaeology
<https://w3id.org/skgo/modsci#Archaeology> rdf:type owl:Class ;
                                           rdfs:subClassOf <https://w3id.org/skgo/modsci#SocialSciences> ;
                                           rdfs:comment "Archaeology, or archeology, is the study of human activity through the recovery and analysis of material culture." ;
                                           rdfs:label "Archaeology" .


###  https://w3id.org/skgo/modsci#Architecture
<https://w3id.org/skgo/modsci#Architecture> rdf:type owl:Class ;
                                            rdfs:subClassOf <https://w3id.org/skgo/modsci#AppliedSciences> ;
                                            rdfs:comment "Architecture is the art and science of designing buildings." ;
                                            rdfs:label "Architecture" .


###  https://w3id.org/skgo/modsci#ArtificialIntelligence
<https://w3id.org/skgo/modsci#ArtificialIntelligence> rdf:type owl:Class ;
                                                      rdfs:subClassOf <https://w3id.org/skgo/modsci#InterdisciplinaryStudies> ;
                                                      rdfs:comment "In computer science, artificial intelligence (AI), sometimes called machine intelligence, is intelligence demonstrated by machines, in contrast to the natural intelligence displayed by humans. Colloquially, the term \"artificial intelligence\" is often used to describe machines (or computers) that mimic \"cognitive\" functions that humans associate with the human mind, such as \"learning\" and \"problem solving\"." ;
                                                      rdfs:label "Artificial Intelligence" .


###  https://w3id.org/skgo/modsci#Astrobiology
<https://w3id.org/skgo/modsci#Astrobiology> rdf:type owl:Class ;
                                            rdfs:subClassOf <https://w3id.org/skgo/modsci#Biology> ;
                                            rdfs:comment "Astrobiology, formerly known as exobiology, is an interdisciplinary scientific field concerned with the origins, early evolution, distribution, and future of life in the universe." ;
                                            rdfs:label "Astrobiology" .


###  https://w3id.org/skgo/modsci#Astrochemistry
<https://w3id.org/skgo/modsci#Astrochemistry> rdf:type owl:Class ;
                                              rdfs:subClassOf <https://w3id.org/skgo/modsci#Chemistry> ;
                                              rdfs:comment "Astrochemistry is the study of the abundance and reactions of molecules in the Universe, and their interaction with radiation." ;
                                              rdfs:label "Astrochemistry" .


###  https://w3id.org/skgo/modsci#Astrometry
<https://w3id.org/skgo/modsci#Astrometry> rdf:type owl:Class ;
                                          rdfs:subClassOf <https://w3id.org/skgo/modsci#Astronomy> ;
                                          rdfs:comment "Astrometry is the study of the positions, distances between, and motions of astronomical objects." ;
                                          rdfs:label "Astrometry" .


###  https://w3id.org/skgo/modsci#Astronomy
<https://w3id.org/skgo/modsci#Astronomy> rdf:type owl:Class ;
                                         rdfs:subClassOf <https://w3id.org/skgo/modsci#NaturalScience> ;
                                         rdfs:comment "is a science involving the observation and explanation of events occurring outside Earth and its atmosphere." ;
                                         rdfs:label "Astronomy" .


###  https://w3id.org/skgo/modsci#AtmosphericSciences
<https://w3id.org/skgo/modsci#AtmosphericSciences> rdf:type owl:Class ;
                                                   rdfs:subClassOf <https://w3id.org/skgo/modsci#EarthScience> ;
                                                   rdfs:comment "Atmospheric science is an umbrella term for the study of the atmosphere and its processes." ;
                                                   rdfs:label "Atmospheric Sciences" .


###  https://w3id.org/skgo/modsci#Atomic
<https://w3id.org/skgo/modsci#Atomic> rdf:type owl:Class ;
                                      rdfs:subClassOf <https://w3id.org/skgo/modsci#Physics> ;
                                      rdfs:comment "Atomic, molecular, and optical physics (AMO) is the study of matter-matter and light-matter interactions; at the scale of one or a few atoms and energy scales around several electron volts." ;
                                      rdfs:label "Atomic, Molecular, and Optical Physics" .


###  https://w3id.org/skgo/modsci#AutomataTheory
<https://w3id.org/skgo/modsci#AutomataTheory> rdf:type owl:Class ;
                                              rdfs:subClassOf <https://w3id.org/skgo/modsci#TheoryOfComputation> ;
                                              rdfs:comment "Automata theory is the study of abstract machines and automata, as well as the computational problems that can be solved using them." ;
                                              rdfs:label "Automata Theory" .


###  https://w3id.org/skgo/modsci#BehaviouralSciences
<https://w3id.org/skgo/modsci#BehaviouralSciences> rdf:type owl:Class ;
                                                   rdfs:subClassOf <https://w3id.org/skgo/modsci#ModernScience> ;
                                                   rdfs:comment "Behavioural sciences explore the cognitive processes within organisms and the behavioural interactions between organisms in the natural world." ;
                                                   rdfs:label "Behavioural Sciences" .


###  https://w3id.org/skgo/modsci#Biochemistry
<https://w3id.org/skgo/modsci#Biochemistry> rdf:type owl:Class ;
                                            rdfs:subClassOf <https://w3id.org/skgo/modsci#Biology> ,
                                                            <https://w3id.org/skgo/modsci#Chemistry> ;
                                            rdfs:comment "Biochemistry is the chemistry of life." ;
                                            rdfs:label "Biochemistry" .


###  https://w3id.org/skgo/modsci#Bioengineering
<https://w3id.org/skgo/modsci#Bioengineering> rdf:type owl:Class ;
                                              rdfs:subClassOf <https://w3id.org/skgo/modsci#Biology> ,
                                                              <https://w3id.org/skgo/modsci#Engineering> ;
                                              rdfs:comment "Biological engineering, or bioengineering/bio-engineering, is the application of principles of biology and the tools of engineering to create usable, tangible, economically viable products." ;
                                              rdfs:label "Biological Engineering" .


###  https://w3id.org/skgo/modsci#Bioethics
<https://w3id.org/skgo/modsci#Bioethics> rdf:type owl:Class ;
                                         rdfs:subClassOf <https://w3id.org/skgo/modsci#Biology> ;
                                         rdfs:comment "Bioethics is the study of the ethical issues emerging from advances in biology and medicine." ;
                                         rdfs:label "Bioethics" .


###  https://w3id.org/skgo/modsci#Biogeography
<https://w3id.org/skgo/modsci#Biogeography> rdf:type owl:Class ;
                                            rdfs:subClassOf <https://w3id.org/skgo/modsci#Biology> ;
                                            rdfs:comment "Biogeography is the study of the distribution of species and ecosystems in geographic space and through geological time." ;
                                            rdfs:label "Biogeography" .


###  https://w3id.org/skgo/modsci#Bioinformatics
<https://w3id.org/skgo/modsci#Bioinformatics> rdf:type owl:Class ;
                                              rdfs:subClassOf <https://w3id.org/skgo/modsci#Biology> ,
                                                              <https://w3id.org/skgo/modsci#InterdisciplinaryStudies> ;
                                              rdfs:comment "Bioinformatics and Computational biology are interdisciplinary fields of research, development and application of algorithms, computational and statistical methods for management and analysis of biological data, and for solving basic biological problems." ;
                                              rdfs:label "Bioinformatics" .


###  https://w3id.org/skgo/modsci#Biology
<https://w3id.org/skgo/modsci#Biology> rdf:type owl:Class ;
                                       rdfs:subClassOf <https://w3id.org/skgo/modsci#NaturalScience> ;
                                       rdfs:comment "Biology is the science of life. It is concerned with the characteristics and behaviors of organisms" ;
                                       rdfs:label "Biology" .


###  https://w3id.org/skgo/modsci#BiomedicalEngineering
<https://w3id.org/skgo/modsci#BiomedicalEngineering> rdf:type owl:Class ;
                                                     rdfs:subClassOf <https://w3id.org/skgo/modsci#InterdisciplinaryStudies> ;
                                                     rdfs:comment "Biomedical engineering (BME) or medical engineering is the application of engineering principles and design concepts to medicine and biology for healthcare purposes (e.g. diagnostic or therapeutic)." ;
                                                     rdfs:label "Biomedical Engineering" .


###  https://w3id.org/skgo/modsci#Biophysics
<https://w3id.org/skgo/modsci#Biophysics> rdf:type owl:Class ;
                                          rdfs:subClassOf <https://w3id.org/skgo/modsci#Biology> ;
                                          rdfs:comment "Biophysics is an interdisciplinary science that applies approaches and methods traditionally used in physics to study biological phenomena." ;
                                          rdfs:label "Biophysics" .


###  https://w3id.org/skgo/modsci#Biopsychology
<https://w3id.org/skgo/modsci#Biopsychology> rdf:type owl:Class ;
                                             rdfs:subClassOf <https://w3id.org/skgo/modsci#Biology> ;
                                             rdfs:comment "Biological psychology,is the application of the principles of biology to the study of physiological and developmental mechanisms of behavior in humans and other animals." ;
                                             rdfs:label "Biopsychology" .


###  https://w3id.org/skgo/modsci#Biostatistics
<https://w3id.org/skgo/modsci#Biostatistics> rdf:type owl:Class ;
                                             rdfs:subClassOf <https://w3id.org/skgo/modsci#Biology> ;
                                             rdfs:comment "Biostatistics are the development and application of statistical methods to a wide range of topics in biology." ;
                                             rdfs:label "Biostatistics" .


###  https://w3id.org/skgo/modsci#Biotechnology
<https://w3id.org/skgo/modsci#Biotechnology> rdf:type owl:Class ;
                                             rdfs:subClassOf <https://w3id.org/skgo/modsci#Biology> ;
                                             rdfs:comment "Biotechnology is a technology based on biology, especially when used in agriculture, food science, medicine, and genetic engineering." ;
                                             rdfs:label "Biotechnology" .


###  https://w3id.org/skgo/modsci#Botany
<https://w3id.org/skgo/modsci#Botany> rdf:type owl:Class ;
                                      rdfs:subClassOf <https://w3id.org/skgo/modsci#Biology> ;
                                      rdfs:comment "Botany also called plant science(s), plant biology or phytology, is the science of plant life and a branch of biology." ;
                                      rdfs:label "Botany" .


###  https://w3id.org/skgo/modsci#CellBiology
<https://w3id.org/skgo/modsci#CellBiology> rdf:type owl:Class ;
                                           rdfs:subClassOf <https://w3id.org/skgo/modsci#Biology> ;
                                           rdfs:comment "Cell biology is a branch of biology that studies the structure and function of the cell, which is the basic unit of life." ;
                                           rdfs:label "Cell Biology" .


###  https://w3id.org/skgo/modsci#ChemicalEngineering
<https://w3id.org/skgo/modsci#ChemicalEngineering> rdf:type owl:Class ;
                                                   rdfs:subClassOf <https://w3id.org/skgo/modsci#Chemistry> ;
                                                   rdfs:comment "Chemical engineering is the application of science, in particular chemistry, fluid physics, and biology, along with mathematics and economics to the human endeavor of converting raw materials or chemicals into more useful or valuable forms." ;
                                                   rdfs:label "Chemical Engineering" .


###  https://w3id.org/skgo/modsci#Chemistry
<https://w3id.org/skgo/modsci#Chemistry> rdf:type owl:Class ;
                                         rdfs:subClassOf <https://w3id.org/skgo/modsci#NaturalScience> ;
                                         rdfs:comment "Chemistry is defined as the science of matter, different from physics, in terms of matter's chemical structure, reactivity, properties and reactions or transformations." ;
                                         rdfs:label "Chemistry" .


###  https://w3id.org/skgo/modsci#CognitiveScience
<https://w3id.org/skgo/modsci#CognitiveScience> rdf:type owl:Class ;
                                                rdfs:subClassOf <https://w3id.org/skgo/modsci#InterdisciplinaryStudies> ;
                                                rdfs:comment "Cognitive science is the interdisciplinary, scientific study of the mind and its processes." ;
                                                rdfs:label "Cognitive Science" .


###  https://w3id.org/skgo/modsci#ColloidalChemistry
<https://w3id.org/skgo/modsci#ColloidalChemistry> rdf:type owl:Class ;
                                                  rdfs:subClassOf <https://w3id.org/skgo/modsci#Chemistry> ;
                                                  rdfs:comment "Interface and colloid science is an interdisciplinary intersection of branches of chemistry, physics, nanoscience and other fields dealing with colloids, heterogeneous systems consisting of a mechanical mixture of particles between 1 nm and 1000 nm dispersed in a continuous medium." ;
                                                  rdfs:label "Colloidal Chemistry" .


###  https://w3id.org/skgo/modsci#CommunicationAndSecurity
<https://w3id.org/skgo/modsci#CommunicationAndSecurity> rdf:type owl:Class ;
                                                        rdfs:subClassOf <https://w3id.org/skgo/modsci#ComputerScience> ;
                                                        rdfs:label "Communication and Security" .


###  https://w3id.org/skgo/modsci#CommunicationStudies
<https://w3id.org/skgo/modsci#CommunicationStudies> rdf:type owl:Class ;
                                                    rdfs:subClassOf <https://w3id.org/skgo/modsci#SocialSciences> ;
                                                    rdfs:comment "Communication is the act of conveying meanings from one entity or group to another through the use of mutually understood signs, symbols, and semiotic rules." ;
                                                    rdfs:label "Communication" .


###  https://w3id.org/skgo/modsci#CompilerTheory
<https://w3id.org/skgo/modsci#CompilerTheory> rdf:type owl:Class ;
                                              rdfs:subClassOf <https://w3id.org/skgo/modsci#ProgrammingLanguages> ;
                                              rdfs:comment "A compiler implements a formal transformation from a high-level source program to a low-level target program." ;
                                              rdfs:label "Compiler Theory" .


###  https://w3id.org/skgo/modsci#ComputabilityTheory
<https://w3id.org/skgo/modsci#ComputabilityTheory> rdf:type owl:Class ;
                                                   rdfs:subClassOf <https://w3id.org/skgo/modsci#TheoryOfComputation> ;
                                                   rdfs:comment "Computability theory, also known as recursion theory, is a branch of mathematical logic, of computer science, and of the theory of computation that originated in the 1930s with the study of computable functions and Turing degrees." ;
                                                   rdfs:label "Computability Theory" .


###  https://w3id.org/skgo/modsci#ComputationalComplexityTheory
<https://w3id.org/skgo/modsci#ComputationalComplexityTheory> rdf:type owl:Class ;
                                                             rdfs:subClassOf <https://w3id.org/skgo/modsci#TheoryOfComputation> ;
                                                             rdfs:comment "Computational complexity theory focuses on classifying computational problems according to their inherent difficulty, and relating these classes to each other. A computational problem is a task solved by a computer." ;
                                                             rdfs:label "Computational Complexity Theory" .


###  https://w3id.org/skgo/modsci#ComputationalLinguistics
<https://w3id.org/skgo/modsci#ComputationalLinguistics> rdf:type owl:Class ;
                                                        rdfs:subClassOf <https://w3id.org/skgo/modsci#InterdisciplinaryStudies> ;
                                                        rdfs:comment "Computational linguistics is an interdisciplinary field concerned with the statistical or rule-based modeling of natural language from a computational perspective, as well as the study of appropriate computational approaches to linguistic questions." ;
                                                        rdfs:label "Computational Linguistics" .


###  https://w3id.org/skgo/modsci#ComputationalPhysics
<https://w3id.org/skgo/modsci#ComputationalPhysics> rdf:type owl:Class ;
                                                    rdfs:subClassOf <https://w3id.org/skgo/modsci#Physics> ;
                                                    rdfs:comment "Computational physics is the study and implementation of numerical algorithms in order to solve problems in physics for which a quantitative theory already exists." ;
                                                    rdfs:label "Computational Physics" .


###  https://w3id.org/skgo/modsci#ComputerArchitecture
<https://w3id.org/skgo/modsci#ComputerArchitecture> rdf:type owl:Class ;
                                                    rdfs:subClassOf <https://w3id.org/skgo/modsci#ComputerScience> ;
                                                    rdfs:comment "In computer engineering, computer architecture is a set of rules and methods that describe the functionality, organization, and implementation of computer systems." ;
                                                    rdfs:label "Computer Architecture" .


###  https://w3id.org/skgo/modsci#ComputerConcurrency
<https://w3id.org/skgo/modsci#ComputerConcurrency> rdf:type owl:Class ;
                                                   rdfs:subClassOf <https://w3id.org/skgo/modsci#DistributedSystems> ;
                                                   rdfs:comment "In computer science, concurrency is the ability of different parts or units of a program, algorithm, or problem to be executed out-of-order or in partial order, without affecting the final outcome. This allows for parallel execution of the concurrent units, which can significantly improve overall speed of the execution in multi-processor and multi-core systems." ;
                                                   rdfs:label "Computer Concurrency" .


###  https://w3id.org/skgo/modsci#ComputerGraphics
<https://w3id.org/skgo/modsci#ComputerGraphics> rdf:type owl:Class ;
                                                rdfs:subClassOf <https://w3id.org/skgo/modsci#Graphics> ;
                                                rdfs:comment "Computer graphics are pictures and films created using computers. Usually, the term refers to computer-generated image data created with the help of specialized graphical hardware and software." ;
                                                rdfs:label "Computer Graphics" .


###  https://w3id.org/skgo/modsci#ComputerScience
<https://w3id.org/skgo/modsci#ComputerScience> rdf:type owl:Class ;
                                               rdfs:subClassOf <https://w3id.org/skgo/modsci#AppliedSciences> ;
                                               rdfs:comment "Computer science is the study of processes that interact with data and that can be represented as data in the form of programs." ;
                                               rdfs:label "Computer Science" .


###  https://w3id.org/skgo/modsci#ComputerSecurity
<https://w3id.org/skgo/modsci#ComputerSecurity> rdf:type owl:Class ;
                                                rdfs:subClassOf <https://w3id.org/skgo/modsci#CommunicationAndSecurity> ;
                                                rdfs:comment "Computer security, cybersecurity or information technology security (IT security) is the protection of computer systems from the theft of or damage to their hardware, software, or electronic data, as well as from the disruption or misdirection of the services they provide." ;
                                                rdfs:label "Computer Security" .


###  https://w3id.org/skgo/modsci#CondensedMatterPhysics
<https://w3id.org/skgo/modsci#CondensedMatterPhysics> rdf:type owl:Class ;
                                                      rdfs:subClassOf <https://w3id.org/skgo/modsci#Physics> ;
                                                      rdfs:comment "Condensed matter physics is the field of physics that deals with the macroscopic physical properties of matter." ;
                                                      rdfs:label "Condensed Matter Physics" .


###  https://w3id.org/skgo/modsci#Cosmology
<https://w3id.org/skgo/modsci#Cosmology> rdf:type owl:Class ;
                                         rdfs:subClassOf <https://w3id.org/skgo/modsci#Astronomy> ;
                                         rdfs:comment "Physical cosmology is the study of the largest-scale structures and dynamics of the Universe and is concerned with fundamental questions about its origin, structure, evolution, and ultimate fate." ;
                                         rdfs:label "Physical Cosmology" .


###  https://w3id.org/skgo/modsci#Cryobiology
<https://w3id.org/skgo/modsci#Cryobiology> rdf:type owl:Class ;
                                           rdfs:subClassOf <https://w3id.org/skgo/modsci#Biology> ;
                                           rdfs:comment "Cryobiology is the study of living organisms, organs, biological tissues or biological cells at low temperatures." ;
                                           rdfs:label "Cryobiology" .


###  https://w3id.org/skgo/modsci#Cryptography
<https://w3id.org/skgo/modsci#Cryptography> rdf:type owl:Class ;
                                            rdfs:subClassOf <https://w3id.org/skgo/modsci#CommunicationAndSecurity> ;
                                            rdfs:comment "Cryptography or cryptology is the practice and study of techniques for secure communication in the presence of third parties called adversaries." ;
                                            rdfs:label "Cryptography" .


###  https://w3id.org/skgo/modsci#Crystallography
<https://w3id.org/skgo/modsci#Crystallography> rdf:type owl:Class ;
                                               rdfs:subClassOf <https://w3id.org/skgo/modsci#Chemistry> ;
                                               rdfs:comment "Crystallography is the scientific study of crystals." ;
                                               rdfs:label "Crystallography" .


###  https://w3id.org/skgo/modsci#CulturalStudies
<https://w3id.org/skgo/modsci#CulturalStudies> rdf:type owl:Class ;
                                               rdfs:subClassOf <https://w3id.org/skgo/modsci#InterdisciplinaryStudies> ;
                                               rdfs:comment "Cultural studies is a field of theoretically, politically, and empirically engaged cultural analysis that concentrates upon the political dynamics of contemporary culture, its historical foundations, defining traits, conflicts, and contingencies." ;
                                               rdfs:label "Cultural Studies" .


###  https://w3id.org/skgo/modsci#Cybernetics
<https://w3id.org/skgo/modsci#Cybernetics> rdf:type owl:Class ;
                                           rdfs:subClassOf <https://w3id.org/skgo/modsci#InterdisciplinaryStudies> ;
                                           rdfs:comment "Cybernetics is a transdisciplinary approach for exploring regulatory systems with feedback, their structures, constraints, and possibilities." ;
                                           rdfs:label "Cybernetics" .


###  https://w3id.org/skgo/modsci#DataMining
<https://w3id.org/skgo/modsci#DataMining> rdf:type owl:Class ;
                                          rdfs:subClassOf <https://w3id.org/skgo/modsci#Databases> ;
                                          rdfs:comment "Data mining is the process of discovering patterns in large data sets involving methods at the intersection of machine learning, statistics, and database systems." ;
                                          rdfs:label "Data Mining" .


###  https://w3id.org/skgo/modsci#Databases
<https://w3id.org/skgo/modsci#Databases> rdf:type owl:Class ;
                                         rdfs:subClassOf <https://w3id.org/skgo/modsci#ComputerScience> ;
                                         rdfs:label "Databases" .


###  https://w3id.org/skgo/modsci#Dentistry
<https://w3id.org/skgo/modsci#Dentistry> rdf:type owl:Class ;
                                         rdfs:subClassOf <https://w3id.org/skgo/modsci#HealthSciences> ;
                                         rdfs:comment "Dentistry, also known as Dental and Oral Medicine, is a branch of medicine that consists of the study, diagnosis, prevention, and treatment of diseases, disorders, and conditions of the oral cavity, commonly in the dentition but also the oral mucosa, and of adjacent and related structures and tissues, particularly in the maxillofacial (jaw and facial) area." ;
                                         rdfs:label "Dentistry" .


###  https://w3id.org/skgo/modsci#DevelopmentalBiology
<https://w3id.org/skgo/modsci#DevelopmentalBiology> rdf:type owl:Class ;
                                                    rdfs:subClassOf <https://w3id.org/skgo/modsci#Biology> ;
                                                    rdfs:comment "Developmental biology is the study of the process by which animals and plants grow and develop." ;
                                                    rdfs:label "Developmental Biology" .


###  https://w3id.org/skgo/modsci#DistributedComputing
<https://w3id.org/skgo/modsci#DistributedComputing> rdf:type owl:Class ;
                                                    rdfs:subClassOf <https://w3id.org/skgo/modsci#DistributedSystems> ;
                                                    rdfs:comment "Distributed computing is a field of computer science that studies distributed systems. A distributed system is a system whose components are located on different networked computers, which communicate and coordinate their actions by passing messages to one another." ;
                                                    rdfs:label "Distributed Computing" .


###  https://w3id.org/skgo/modsci#DistributedSystems
<https://w3id.org/skgo/modsci#DistributedSystems> rdf:type owl:Class ;
                                                  rdfs:subClassOf <https://w3id.org/skgo/modsci#ComputerScience> ;
                                                  rdfs:label "Concurrent, Parallel, and Distributed systems" .


###  https://w3id.org/skgo/modsci#EarthScience
<https://w3id.org/skgo/modsci#EarthScience> rdf:type owl:Class ;
                                            rdfs:subClassOf <https://w3id.org/skgo/modsci#NaturalScience> ;
                                            rdfs:comment "Earth science (also known as geoscience, the geosciences, or the Earth sciences) includes all the sciences related to the planet Earth." ;
                                            rdfs:label "Earth Science" .


###  https://w3id.org/skgo/modsci#Ecology
<https://w3id.org/skgo/modsci#Ecology> rdf:type owl:Class ;
                                       rdfs:subClassOf <https://w3id.org/skgo/modsci#Biology> ,
                                                       <https://w3id.org/skgo/modsci#EarthScience> ;
                                       rdfs:comment "Ecology is the branch of science that studies the distribution and interactions between living things and the physical environment." ;
                                       rdfs:label "Ecology" .


###  https://w3id.org/skgo/modsci#Economics
<https://w3id.org/skgo/modsci#Economics> rdf:type owl:Class ;
                                         rdfs:subClassOf <https://w3id.org/skgo/modsci#SocialSciences> ;
                                         rdfs:comment "Economics is the social science that studies the production, distribution, and consumption of goods and services." ;
                                         rdfs:label "Economics" .


###  https://w3id.org/skgo/modsci#Education
<https://w3id.org/skgo/modsci#Education> rdf:type owl:Class ;
                                         rdfs:subClassOf <https://w3id.org/skgo/modsci#AppliedSciences> ;
                                         rdfs:comment "Education is the teaching or learning of knowledge, especially to develop the reasoning, judgement and skill required in adult life and professional occupations." ;
                                         rdfs:label "Education" .


###  https://w3id.org/skgo/modsci#Engineering
<https://w3id.org/skgo/modsci#Engineering> rdf:type owl:Class ;
                                           rdfs:subClassOf <https://w3id.org/skgo/modsci#AppliedSciences> ;
                                           rdfs:comment "Engineering is the practical application of science. This is accomplished through knowledge, mathematics, and practical experience applied to the design of useful objects or processes." ;
                                           rdfs:label "Engineering" .


###  https://w3id.org/skgo/modsci#EnvironmentalChemistry
<https://w3id.org/skgo/modsci#EnvironmentalChemistry> rdf:type owl:Class ;
                                                      rdfs:subClassOf <https://w3id.org/skgo/modsci#Chemistry> ;
                                                      rdfs:comment "Environmental chemistry is the scientific study of the physical, chemical and biochemical properties and processes of polluting substances in the environment." ;
                                                      rdfs:label "Environmental Chemistry" .


###  https://w3id.org/skgo/modsci#EnvironmentalScience
<https://w3id.org/skgo/modsci#EnvironmentalScience> rdf:type owl:Class ;
                                                    rdfs:subClassOf <https://w3id.org/skgo/modsci#EarthScience> ;
                                                    rdfs:comment "Environmental science is the science of the interactions between the physical, chemical, and biological components of the environment, but with particular attention to the effects of humans on the natural environment." ;
                                                    rdfs:label "Environmental Science" .


###  https://w3id.org/skgo/modsci#Epidemiology
<https://w3id.org/skgo/modsci#Epidemiology> rdf:type owl:Class ;
                                            rdfs:subClassOf <https://w3id.org/skgo/modsci#HealthSciences> ;
                                            rdfs:comment "Epidemiology is the study and analysis of the distribution (who, when, and where), patterns and determinants of health and disease conditions in defined populations." ;
                                            rdfs:label "Epidemiology" .


###  https://w3id.org/skgo/modsci#Ergonomics
<https://w3id.org/skgo/modsci#Ergonomics> rdf:type owl:Class ;
                                          rdfs:subClassOf <https://w3id.org/skgo/modsci#AppliedSciences> ;
                                          rdfs:comment "Human factors and ergonomics is the application of psychological and physiological principles to the (engineering and) design of products, processes, and systems." ;
                                          rdfs:label "Ergonomics" .


###  https://w3id.org/skgo/modsci#EthnicStudies
<https://w3id.org/skgo/modsci#EthnicStudies> rdf:type owl:Class ;
                                             rdfs:subClassOf <https://w3id.org/skgo/modsci#InterdisciplinaryStudies> ;
                                             rdfs:comment "Ethnic studies, in the United States, is the interdisciplinary study of difference—chiefly race, ethnicity, and nation, but also sexuality, gender, and other such markings—and power, as expressed by the state, by civil society, and by individuals." ;
                                             rdfs:label "Ethnic Studies" .


###  https://w3id.org/skgo/modsci#Ethnobiology
<https://w3id.org/skgo/modsci#Ethnobiology> rdf:type owl:Class ;
                                            rdfs:subClassOf <https://w3id.org/skgo/modsci#Biology> ;
                                            rdfs:comment "Ethnobiology is the scientific study of the way living things are treated or used by different human cultures." ;
                                            rdfs:label "Ethnobiology" .


###  https://w3id.org/skgo/modsci#Ethnology
<https://w3id.org/skgo/modsci#Ethnology> rdf:type owl:Class ;
                                         rdfs:subClassOf <https://w3id.org/skgo/modsci#SocialSciences> ;
                                         rdfs:comment "Ethnology is the science that analyzes human cultures and compares them." ;
                                         rdfs:label "Ethnology" .


###  https://w3id.org/skgo/modsci#Ethology
<https://w3id.org/skgo/modsci#Ethology> rdf:type owl:Class ;
                                        rdfs:subClassOf <https://w3id.org/skgo/modsci#BehaviouralSciences> ;
                                        rdfs:comment "Ethology is the scientific and objective study of animal behaviour, usually with a focus on behaviour under natural conditions, and viewing behaviour as an evolutionarily adaptive trait." ;
                                        rdfs:label "Ethology" .


###  https://w3id.org/skgo/modsci#EvolutionaryBiology
<https://w3id.org/skgo/modsci#EvolutionaryBiology> rdf:type owl:Class ;
                                                   rdfs:subClassOf <https://w3id.org/skgo/modsci#Biology> ;
                                                   rdfs:comment "Evolutionary biology is a sub-field of biology concerned with the study of the evolutionary processes that produced the diversity of life on Earth." ;
                                                   rdfs:label "Evolutionary Biology" .


###  https://w3id.org/skgo/modsci#EvolutionaryPsychology
<https://w3id.org/skgo/modsci#EvolutionaryPsychology> rdf:type owl:Class ;
                                                      rdfs:subClassOf <https://w3id.org/skgo/modsci#InterdisciplinaryStudies> ;
                                                      rdfs:comment "Evolutionary psychology is a theoretical approach in the social and natural sciences that examines psychological structure from a modern evolutionary perspective." ;
                                                      rdfs:label "Evolutionary Psychology" .


###  https://w3id.org/skgo/modsci#ExperimentalPhysics
<https://w3id.org/skgo/modsci#ExperimentalPhysics> rdf:type owl:Class ;
                                                   rdfs:subClassOf <https://w3id.org/skgo/modsci#Physics> ;
                                                   rdfs:comment "Experimental physics is the category of disciplines and sub-disciplines in the field of physics that are concerned with the observation of physical phenomena and experiments." ;
                                                   rdfs:label "Experimental Physics" .


###  https://w3id.org/skgo/modsci#ExtragalacticAstronomy
<https://w3id.org/skgo/modsci#ExtragalacticAstronomy> rdf:type owl:Class ;
                                                      rdfs:subClassOf <https://w3id.org/skgo/modsci#Astronomy> ;
                                                      rdfs:comment "It is the study of all astronomical objects which are not covered by galactic astronomy." ;
                                                      rdfs:label "Extragalactic Astronomy" .


###  https://w3id.org/skgo/modsci#FoodChemistry
<https://w3id.org/skgo/modsci#FoodChemistry> rdf:type owl:Class ;
                                             rdfs:subClassOf <https://w3id.org/skgo/modsci#Chemistry> ;
                                             rdfs:comment "Food chemistry is the study of chemical processes and interactions of all biological and non-biological components of foods." ;
                                             rdfs:label "Food Chemistry" .


###  https://w3id.org/skgo/modsci#Forensics
<https://w3id.org/skgo/modsci#Forensics> rdf:type owl:Class ;
                                         rdfs:subClassOf <https://w3id.org/skgo/modsci#AppliedSciences> ;
                                         rdfs:comment "Forensic science, also known as criminalistics, is the application of science to criminal and civil laws, mainly—on the criminal side—during criminal investigation, as governed by the legal standards of admissible evidence and criminal procedure." ;
                                         rdfs:label "Forensics" .


###  https://w3id.org/skgo/modsci#Forestry
<https://w3id.org/skgo/modsci#Forestry> rdf:type owl:Class ;
                                        rdfs:subClassOf <https://w3id.org/skgo/modsci#Biology> ;
                                        rdfs:comment "Forestry is the art, science, and practice of studying and managing forests and related natural resources." ;
                                        rdfs:label "Forestry" .


###  https://w3id.org/skgo/modsci#FormalScience
<https://w3id.org/skgo/modsci#FormalScience> rdf:type owl:Class ;
                                             rdfs:subClassOf <https://w3id.org/skgo/modsci#ModernScience> ;
                                             rdfs:comment "Formal sciences are a branch of science studying formal language disciplines concerned with formal systems, such as logic, mathematics, statistics, theoretical computer science, artificial intelligence, information theory, game theory, systems theory, decision theory, and theoretical linguistics." ;
                                             rdfs:label "Formal Science" .


###  https://w3id.org/skgo/modsci#GalacticAstronomy
<https://w3id.org/skgo/modsci#GalacticAstronomy> rdf:type owl:Class ;
                                                 rdfs:subClassOf <https://w3id.org/skgo/modsci#Astronomy> ;
                                                 rdfs:comment "The study of everything outside our galaxy, including all other galaxies." ;
                                                 rdfs:label "Galactic Astronomy" .


###  https://w3id.org/skgo/modsci#Genetics
<https://w3id.org/skgo/modsci#Genetics> rdf:type owl:Class ;
                                        rdfs:subClassOf <https://w3id.org/skgo/modsci#Biology> ;
                                        rdfs:comment "Genetics is the study of genes, heredity, and the variation of organisms, as well as the medical practice of diagnosing, treating, and counseling patients with genetic disorders." ;
                                        rdfs:label "Genetics" .


###  https://w3id.org/skgo/modsci#Geochemistry
<https://w3id.org/skgo/modsci#Geochemistry> rdf:type owl:Class ;
                                            rdfs:subClassOf <https://w3id.org/skgo/modsci#Chemistry> ;
                                            rdfs:comment "Geochemistry is the science that uses the tools and principles of chemistry to explain the mechanisms behind major geological systems such as the Earth's crust and its oceans." ;
                                            rdfs:label "Geochemistry" .


###  https://w3id.org/skgo/modsci#Geodesy
<https://w3id.org/skgo/modsci#Geodesy> rdf:type owl:Class ;
                                       rdfs:subClassOf <https://w3id.org/skgo/modsci#EarthScience> ;
                                       rdfs:comment "Geodesy is the Earth science of accurately measuring and understanding Earth's geometric shape, orientation in space and gravitational field." ;
                                       rdfs:label "Geodesy" .


###  https://w3id.org/skgo/modsci#Geography
<https://w3id.org/skgo/modsci#Geography> rdf:type owl:Class ;
                                         rdfs:subClassOf <https://w3id.org/skgo/modsci#EarthScience> ;
                                         rdfs:comment "Geography is a field of science devoted to the study of the lands, features, inhabitants, and phenomena of the Earth and planets." ;
                                         rdfs:label "Geography" .


###  https://w3id.org/skgo/modsci#GeologicalSciences
<https://w3id.org/skgo/modsci#GeologicalSciences> rdf:type owl:Class ;
                                                  rdfs:subClassOf <https://w3id.org/skgo/modsci#NaturalScience> ;
                                                  rdfs:label "Geological Sciences" .


###  https://w3id.org/skgo/modsci#Geology
<https://w3id.org/skgo/modsci#Geology> rdf:type owl:Class ;
                                       rdfs:subClassOf <https://w3id.org/skgo/modsci#EarthScience> ;
                                       rdfs:comment "Geology is an earth science concerned with the solid Earth, the rocks of which it is composed, and the processes by which they change over time." ;
                                       rdfs:label "Geology" .


###  https://w3id.org/skgo/modsci#Geomorphology
<https://w3id.org/skgo/modsci#Geomorphology> rdf:type owl:Class ;
                                             rdfs:subClassOf <https://w3id.org/skgo/modsci#EarthScience> ;
                                             rdfs:comment "Geomorphology is the science of surface features and landforms including the forces and processes that create them." ;
                                             rdfs:label "Geomorphology" .


###  https://w3id.org/skgo/modsci#Geophysics
<https://w3id.org/skgo/modsci#Geophysics> rdf:type owl:Class ;
                                          rdfs:subClassOf <https://w3id.org/skgo/modsci#EarthScience> ;
                                          rdfs:comment "Geophysics the physics of the Earth and its environment in space, and study of earth sciences using quantitative physics methods." ;
                                          rdfs:label "Geophysics" .


###  https://w3id.org/skgo/modsci#Gerontology
<https://w3id.org/skgo/modsci#Gerontology> rdf:type owl:Class ;
                                           rdfs:subClassOf <https://w3id.org/skgo/modsci#Biology> ;
                                           rdfs:comment "Gerontology is the study of the social, cultural, psychological, cognitive, and biological aspects of ageing." ;
                                           rdfs:label "Gerontology" .


###  https://w3id.org/skgo/modsci#Glaciology
<https://w3id.org/skgo/modsci#Glaciology> rdf:type owl:Class ;
                                          rdfs:subClassOf <https://w3id.org/skgo/modsci#EarthScience> ;
                                          rdfs:comment "Glaciology is the scientific study of glaciers, or more generally ice and natural phenomena that involve ice." ;
                                          rdfs:label "Glaciology" .


###  https://w3id.org/skgo/modsci#Graphics
<https://w3id.org/skgo/modsci#Graphics> rdf:type owl:Class ;
                                        rdfs:subClassOf <https://w3id.org/skgo/modsci#ComputerScience> ;
                                        rdfs:label "Graphics" .


###  https://w3id.org/skgo/modsci#GreenChemistry
<https://w3id.org/skgo/modsci#GreenChemistry> rdf:type owl:Class ;
                                              rdfs:subClassOf <https://w3id.org/skgo/modsci#Chemistry> ;
                                              rdfs:comment "Green chemistry is the use of chemistry for pollutant source reduction; the definition encompasses therefore all aspects of chemical processes that reduce impact on human health and on the environment." ;
                                              rdfs:label "Green Chemistry" .


###  https://w3id.org/skgo/modsci#Health
<https://w3id.org/skgo/modsci#Health> rdf:type owl:Class ;
                                      rdfs:subClassOf <https://w3id.org/skgo/modsci#InterdisciplinaryStudies> ;
                                      rdfs:comment "Health is a state of physical, mental and social well-being in which disease and infirmity are absent." ;
                                      rdfs:label "Health" .


###  https://w3id.org/skgo/modsci#HealthSciences
<https://w3id.org/skgo/modsci#HealthSciences> rdf:type owl:Class ;
                                              rdfs:subClassOf <https://w3id.org/skgo/modsci#ModernScience> ;
                                              rdfs:comment "Health sciences are those sciences which focus on health, or health care, as core parts of their subject matter." ;
                                              rdfs:label "Health Sciences" .


###  https://w3id.org/skgo/modsci#Healthcare
<https://w3id.org/skgo/modsci#Healthcare> rdf:type owl:Class ;
                                          rdfs:subClassOf <https://w3id.org/skgo/modsci#HealthSciences> ;
                                          rdfs:comment "Health care is the maintenance or improvement of health via the prevention, diagnosis, and treatment of disease, illness, injury, and other physical and mental impairments in people." ;
                                          rdfs:label "Healthcare" .


###  https://w3id.org/skgo/modsci#History
<https://w3id.org/skgo/modsci#History> rdf:type owl:Class ;
                                       rdfs:subClassOf <https://w3id.org/skgo/modsci#FormalScience> ;
                                       rdfs:comment "The history of science is the study of the development of science and scientific knowledge, including both the natural and social sciences (the history of the arts and humanities is termed history of scholarship)." ;
                                       rdfs:label "History of Science" .


###  https://w3id.org/skgo/modsci#HumanComputerInteraction
<https://w3id.org/skgo/modsci#HumanComputerInteraction> rdf:type owl:Class ;
                                                        rdfs:subClassOf <https://w3id.org/skgo/modsci#SoftwareEngineering> ;
                                                        rdfs:comment "Human–computer interaction (HCI) researches the design and use of computer technology, focused on the interfaces between people (users) and computers. Researchers in the field of HCI observe the ways in which humans interact with computers and design technologies that let humans interact with computers in novel ways." ;
                                                        rdfs:label "Human Computer Interaction" .


###  https://w3id.org/skgo/modsci#HumanSciences
<https://w3id.org/skgo/modsci#HumanSciences> rdf:type owl:Class ;
                                             rdfs:subClassOf <https://w3id.org/skgo/modsci#InterdisciplinaryStudies> ;
                                             rdfs:comment "Human science is a term applied to the investigation of human life and activities by a rational, systematic and verifiable methodology that acknowledges the validity of both data derived by impartial observation of sensory experience (objective phenomena) and data derived by means of impartial observation of psychological experience (subjective phenomena)." ;
                                             rdfs:label "Human Sciences" .


###  https://w3id.org/skgo/modsci#Hydrology
<https://w3id.org/skgo/modsci#Hydrology> rdf:type owl:Class ;
                                         rdfs:subClassOf <https://w3id.org/skgo/modsci#EarthScience> ;
                                         rdfs:comment "Hydrology is the scientific study of the movement, distribution, and quality of water on Earth and other planets, including the water cycle, water resources and environmental watershed sustainability." ;
                                         rdfs:label "Hydrology" .


###  https://w3id.org/skgo/modsci#ImageProcessing
<https://w3id.org/skgo/modsci#ImageProcessing> rdf:type owl:Class ;
                                               rdfs:subClassOf <https://w3id.org/skgo/modsci#Graphics> ;
                                               rdfs:comment "In computer science, digital image processing is the use of computer algorithms to perform image processing on digital images." ;
                                               rdfs:label "Image Processing" .


###  https://w3id.org/skgo/modsci#Immunology
<https://w3id.org/skgo/modsci#Immunology> rdf:type owl:Class ;
                                          rdfs:subClassOf <https://w3id.org/skgo/modsci#Biology> ;
                                          rdfs:comment "Immunology is the study of the immune system and its reaction to pathogens, as well as its malfunctions (autoimmune diseases, allergies, rejection of organ transplants, immune deficiency)." ;
                                          rdfs:label "Immunology" .


###  https://w3id.org/skgo/modsci#IndustrialScience
<https://w3id.org/skgo/modsci#IndustrialScience> rdf:type owl:Class ;
                                                 rdfs:subClassOf <https://w3id.org/skgo/modsci#AppliedSciences> ;
                                                 rdfs:comment "An industrial process alters materials or substances." ;
                                                 rdfs:label "Industrial Process" .


###  https://w3id.org/skgo/modsci#InformationScience
<https://w3id.org/skgo/modsci#InformationScience> rdf:type owl:Class ;
                                                  rdfs:subClassOf <https://w3id.org/skgo/modsci#AppliedSciences> ;
                                                  rdfs:comment "Information science is a field primarily concerned with the analysis, collection, classification, manipulation, storage, retrieval, movement, dissemination, and protection of information." ;
                                                  rdfs:label "Information Science" .


###  https://w3id.org/skgo/modsci#InformationVisualization
<https://w3id.org/skgo/modsci#InformationVisualization> rdf:type owl:Class ;
                                                        rdfs:subClassOf <https://w3id.org/skgo/modsci#Graphics> ;
                                                        rdfs:comment "Information visualization or information visualisation is the study of (interactive) visual representations of abstract data to reinforce human cognition." ;
                                                        rdfs:label "Information Visualization" .


###  https://w3id.org/skgo/modsci#InorganicChemistry
<https://w3id.org/skgo/modsci#InorganicChemistry> rdf:type owl:Class ;
                                                  rdfs:subClassOf <https://w3id.org/skgo/modsci#Chemistry> ;
                                                  rdfs:comment "Inorganic chemistry is a catch-all discipline that covers everything in chemistry that is not organic chemistry." ;
                                                  rdfs:label "Inorganic Chemistry" .


###  https://w3id.org/skgo/modsci#InterdisciplinaryStudies
<https://w3id.org/skgo/modsci#InterdisciplinaryStudies> rdf:type owl:Class ;
                                                        rdfs:subClassOf <https://w3id.org/skgo/modsci#ModernScience> ;
                                                        rdfs:comment "Interdisciplinarity or interdisciplinary studies involves the combining of two or more academic disciplines into one activity (e.g., a research project)." ;
                                                        rdfs:label "Interdisciplinary Studies" .


###  https://w3id.org/skgo/modsci#LibraryScience
<https://w3id.org/skgo/modsci#LibraryScience> rdf:type owl:Class ;
                                              rdfs:subClassOf <https://w3id.org/skgo/modsci#AppliedSciences> ,
                                                              <https://w3id.org/skgo/modsci#InterdisciplinaryStudies> ;
                                              rdfs:comment "Library science is an interdisciplinary or multidisciplinary field that applies the practices, perspectives, and tools of management, information technology, education, and other areas to libraries; the collection, organization, preservation, and dissemination of information resources; and the political economy of information." ;
                                              rdfs:label "Library Science" .


###  https://w3id.org/skgo/modsci#Limnology
<https://w3id.org/skgo/modsci#Limnology> rdf:type owl:Class ;
                                         rdfs:subClassOf <https://w3id.org/skgo/modsci#Biology> ,
                                                         <https://w3id.org/skgo/modsci#EarthScience> ;
                                         rdfs:comment "Limnology is a discipline that concerns the study of fresh waters, specifically natural and constructed lakes, ponds, streams, and rivers," ;
                                         rdfs:label "Limnology" .


###  https://w3id.org/skgo/modsci#Linguistics
<https://w3id.org/skgo/modsci#Linguistics> rdf:type owl:Class ;
                                           rdfs:subClassOf <https://w3id.org/skgo/modsci#SocialSciences> ;
                                           rdfs:comment "Linguistics is the scientific study of language." ;
                                           rdfs:label "Linguistics" .


###  https://w3id.org/skgo/modsci#Logic
<https://w3id.org/skgo/modsci#Logic> rdf:type owl:Class ;
                                     rdfs:subClassOf <https://w3id.org/skgo/modsci#InterdisciplinaryStudies> ;
                                     rdfs:comment "Logic is the study of reasoning, or the study of the principles and criteria of valid inference and demonstration." ;
                                     rdfs:label "Logic" .


###  https://w3id.org/skgo/modsci#MarineBiology
<https://w3id.org/skgo/modsci#MarineBiology> rdf:type owl:Class ;
                                             rdfs:subClassOf <https://w3id.org/skgo/modsci#Biology> ;
                                             rdfs:comment "Marine biology is the scientific study of organisms that live in the ocean" ;
                                             rdfs:label "Marine Biology" .


###  https://w3id.org/skgo/modsci#MaterialsScience
<https://w3id.org/skgo/modsci#MaterialsScience> rdf:type owl:Class ;
                                                rdfs:subClassOf <https://w3id.org/skgo/modsci#Chemistry> ;
                                                rdfs:comment "The interdisciplinary field of materials science is the design and discovery of new materials, particularly solids." ;
                                                rdfs:label "Materials Science" .


###  https://w3id.org/skgo/modsci#MathematicalAndTheoreticalBiology
<https://w3id.org/skgo/modsci#MathematicalAndTheoreticalBiology> rdf:type owl:Class ;
                                                                 rdfs:subClassOf <https://w3id.org/skgo/modsci#Biology> ;
                                                                 rdfs:comment "Mathematical and theoretical biology is a branch of biology which employs theoretical analysis, mathematical models and abstractions of the living organisms to investigate the principles that govern the structure, development and behavior of the systems" ;
                                                                 rdfs:label "Mathematical and Theoretical Biology" .


###  https://w3id.org/skgo/modsci#MathematicalPhysics
<https://w3id.org/skgo/modsci#MathematicalPhysics> rdf:type owl:Class ;
                                                   rdfs:subClassOf <https://w3id.org/skgo/modsci#InterdisciplinaryStudies> ;
                                                   rdfs:comment "Mathematical physics refers to the development of mathematical methods for application to problems in physics." ;
                                                   rdfs:label "Mathematical Physics" .


###  https://w3id.org/skgo/modsci#Mathematics
<https://w3id.org/skgo/modsci#Mathematics> rdf:type owl:Class ;
                                           rdfs:subClassOf <https://w3id.org/skgo/modsci#FormalScience> ;
                                           rdfs:comment "Mathematics (colloquially, maths, or math), is the body of knowledge centered on concepts such as quantity, structure, space, and change, and also the academic discipline that studies them." ;
                                           rdfs:label "Mathematics" .


###  https://w3id.org/skgo/modsci#Measurement
<https://w3id.org/skgo/modsci#Measurement> rdf:type owl:Class ;
                                           rdfs:subClassOf <https://w3id.org/skgo/modsci#AppliedSciences> ;
                                           rdfs:comment "Measurement is the assignment of a number to a characteristic of an object or event, which can be compared with other objects or events." ;
                                           rdfs:label "Measurement" .


###  https://w3id.org/skgo/modsci#Mechanics
<https://w3id.org/skgo/modsci#Mechanics> rdf:type owl:Class ;
                                         rdfs:subClassOf <https://w3id.org/skgo/modsci#Physics> ;
                                         rdfs:comment "Mechanics is the branch of science concerned with the behavior of physical bodies when subjected to forces or displacements, and the subsequent effects of the bodies on their environment." ;
                                         rdfs:label "Mechanics" .


###  https://w3id.org/skgo/modsci#MedicinalChemistry
<https://w3id.org/skgo/modsci#MedicinalChemistry> rdf:type owl:Class ;
                                                  rdfs:subClassOf <https://w3id.org/skgo/modsci#Chemistry> ;
                                                  rdfs:comment "Medicinal chemistry and pharmaceutical chemistry are disciplines at the intersection of chemistry, especially synthetic organic chemistry, and pharmacology and various other biological specialties, where they are involved with design, chemical synthesis and development for market of pharmaceutical agents, or bio-active molecules (drugs)." ;
                                                  rdfs:label "Medicinal Chemistry" .


###  https://w3id.org/skgo/modsci#Medicine
<https://w3id.org/skgo/modsci#Medicine> rdf:type owl:Class ;
                                        rdfs:subClassOf <https://w3id.org/skgo/modsci#HealthSciences> ;
                                        rdfs:comment "Medicine is a branch of health science concerned with maintaining human health and restoring it by treating disease and injury; it is both an area of knowledge, a science of body systems and diseases and their treatment, and the applied practice of that knowledge." ;
                                        rdfs:label "Medicine" .


###  https://w3id.org/skgo/modsci#Metabolism
<https://w3id.org/skgo/modsci#Metabolism> rdf:type owl:Class ;
                                          rdfs:subClassOf <https://w3id.org/skgo/modsci#Biology> ;
                                          rdfs:comment "Metabolism is the set of life-sustaining chemical reactions in organisms." ;
                                          rdfs:label "Metabolism" .


###  https://w3id.org/skgo/modsci#Metallurgy
<https://w3id.org/skgo/modsci#Metallurgy> rdf:type owl:Class ;
                                          rdfs:subClassOf <https://w3id.org/skgo/modsci#Chemistry> ;
                                          rdfs:comment "Metallurgy is a domain of materials science and engineering that studies the physical and chemical behavior of metallic elements, their inter-metallic compounds, and their mixtures, which are called alloys." ;
                                          rdfs:label "Metallurgy" .


###  https://w3id.org/skgo/modsci#Metrology
<https://w3id.org/skgo/modsci#Metrology> rdf:type owl:Class ;
                                         rdfs:subClassOf <https://w3id.org/skgo/modsci#AppliedSciences> ;
                                         rdfs:comment "Metrology is the science of measurement." ;
                                         rdfs:label "Metrology" .


###  https://w3id.org/skgo/modsci#MilitaryScience
<https://w3id.org/skgo/modsci#MilitaryScience> rdf:type owl:Class ;
                                               rdfs:subClassOf <https://w3id.org/skgo/modsci#AppliedSciences> ;
                                               rdfs:comment "Military science is the study of military processes, dentsciitutions, and behavior, along with the study of warfare, and the theory and application of organized coercive force." ;
                                               rdfs:label "Military Science" .


###  https://w3id.org/skgo/modsci#ModernScience
<https://w3id.org/skgo/modsci#ModernScience> rdf:type owl:Class ;
                                             rdfs:comment "Science is a systematic enterprise that builds and organizes knowledge in the form of testable explanations and predictions about the universe." ;
                                             rdfs:label "Science" .


###  https://w3id.org/skgo/modsci#MolecularBiology
<https://w3id.org/skgo/modsci#MolecularBiology> rdf:type owl:Class ;
                                                rdfs:subClassOf <https://w3id.org/skgo/modsci#Biology> ;
                                                rdfs:comment "Molecular biology is the study of biology at a molecular level." ;
                                                rdfs:label "Molecular Biology" .


###  https://w3id.org/skgo/modsci#MolecularPhysics
<https://w3id.org/skgo/modsci#MolecularPhysics> rdf:type owl:Class ;
                                                rdfs:subClassOf <https://w3id.org/skgo/modsci#Chemistry> ;
                                                rdfs:comment "Molecular physics deals with the physics and chemistry of molecules." ;
                                                rdfs:label "Molecular Physics" .


###  https://w3id.org/skgo/modsci#Museology
<https://w3id.org/skgo/modsci#Museology> rdf:type owl:Class ;
                                         rdfs:subClassOf <https://w3id.org/skgo/modsci#InterdisciplinaryStudies> ;
                                         rdfs:comment "Museology or museum studies is the study of museums. It explores the history of museums and their role in society, as well as the activities they engage in, including curating, preservation, public programming, and education." ;
                                         rdfs:label "Museology" .


###  https://w3id.org/skgo/modsci#NaturalLanguageProcessing
<https://w3id.org/skgo/modsci#NaturalLanguageProcessing> rdf:type owl:Class ;
                                                         rdfs:subClassOf <https://w3id.org/skgo/modsci#ArtificialIntelligence> ,
                                                                         <https://w3id.org/skgo/modsci#ComputerScience> ,
                                                                         <https://w3id.org/skgo/modsci#Linguistics> ;
                                                         rdfs:comment "Natural language processing (NLP) is a subfield of linguistics, computer science, information engineering, and artificial intelligence concerned with the interactions between computers and human (natural) languages, in particular how to program computers to process and analyze large amounts of natural language data." ;
                                                         rdfs:label "Natural language processing (NLP)" .


###  https://w3id.org/skgo/modsci#NaturalScience
<https://w3id.org/skgo/modsci#NaturalScience> rdf:type owl:Class ;
                                              rdfs:subClassOf <https://w3id.org/skgo/modsci#ModernScience> ;
                                              rdfs:comment "The natural sciences are those branches of empirical science that produce a comprehension of the natural world through the use of data collected from it by observation and measurement to construct deterministic and/or stochastic quantitative models of its phenomena." ;
                                              rdfs:label "Natural Sciences" .


###  https://w3id.org/skgo/modsci#Networking
<https://w3id.org/skgo/modsci#Networking> rdf:type owl:Class ;
                                          rdfs:subClassOf <https://w3id.org/skgo/modsci#CommunicationAndSecurity> ;
                                          rdfs:comment "A computer network is a digital telecommunications network which allows nodes to share resources." ;
                                          rdfs:label "Networking" .


###  https://w3id.org/skgo/modsci#NeuralEngineering
<https://w3id.org/skgo/modsci#NeuralEngineering> rdf:type owl:Class ;
                                                 rdfs:subClassOf <https://w3id.org/skgo/modsci#InterdisciplinaryStudies> ;
                                                 rdfs:comment "Neural engineering is a discipline within biomedical engineering that uses engineering techniques to understand, repair, replace, or enhance neural systems." ;
                                                 rdfs:label "Neural Engineering" .


###  https://w3id.org/skgo/modsci#Neuroscience
<https://w3id.org/skgo/modsci#Neuroscience> rdf:type owl:Class ;
                                            rdfs:subClassOf <https://w3id.org/skgo/modsci#Biology> ,
                                                            <https://w3id.org/skgo/modsci#InterdisciplinaryStudies> ;
                                            rdfs:comment "Neuroscience is a field of study which deals with the structure, development, genetics, biochemistry, physiology, pharmacology and pathology of the nervous system." ;
                                            rdfs:label "Neuroscience" .


###  https://w3id.org/skgo/modsci#NuclearChemistry
<https://w3id.org/skgo/modsci#NuclearChemistry> rdf:type owl:Class ;
                                                rdfs:subClassOf <https://w3id.org/skgo/modsci#Chemistry> ;
                                                rdfs:comment "Nuclear chemistry is the subfield of chemistry dealing with radioactivity, nuclear processes, and transformations in the nuclei of atoms, such as nuclear transmutation and nuclear properties." ;
                                                rdfs:label "Nuclear Chemistry" .


###  https://w3id.org/skgo/modsci#Nursing
<https://w3id.org/skgo/modsci#Nursing> rdf:type owl:Class ;
                                       rdfs:subClassOf <https://w3id.org/skgo/modsci#HealthSciences> ;
                                       rdfs:comment "Nursing is a profession within the health care sector focused on the care of individuals, families, and communities so they may attain, maintain, or recover optimal health and quality of life." ;
                                       rdfs:label "Nursing" .


###  https://w3id.org/skgo/modsci#Oceanography
<https://w3id.org/skgo/modsci#Oceanography> rdf:type owl:Class ;
                                            rdfs:subClassOf <https://w3id.org/skgo/modsci#EarthScience> ;
                                            rdfs:comment "Oceanography also known as oceanology, is the study of the physical and biological aspects of the ocean." ;
                                            rdfs:label "Oceanography" .


###  https://w3id.org/skgo/modsci#OperatingSystems
<https://w3id.org/skgo/modsci#OperatingSystems> rdf:type owl:Class ;
                                                rdfs:subClassOf <https://w3id.org/skgo/modsci#ComputerScience> ;
                                                rdfs:comment "An operating system (OS) is system software that manages computer hardware, software resources, and provides common services for computer programs." ;
                                                rdfs:label "Operating Systems" .


###  https://w3id.org/skgo/modsci#Optics
<https://w3id.org/skgo/modsci#Optics> rdf:type owl:Class ;
                                      rdfs:subClassOf <https://w3id.org/skgo/modsci#AppliedSciences> ;
                                      rdfs:comment "Optics is the branch of physics that studies the behaviour and properties of light, including its interactions with matter and the construction of instruments that use or detect it." ;
                                      rdfs:label "Optics" .


###  https://w3id.org/skgo/modsci#OrganicChemistry
<https://w3id.org/skgo/modsci#OrganicChemistry> rdf:type owl:Class ;
                                                rdfs:subClassOf <https://w3id.org/skgo/modsci#Chemistry> ;
                                                rdfs:comment "Organic chemistry is the study of organic, or carbon based, molecules." ;
                                                rdfs:label "Organic Chemistry" .


###  https://w3id.org/skgo/modsci#OrganometallicChemistry
<https://w3id.org/skgo/modsci#OrganometallicChemistry> rdf:type owl:Class ;
                                                       rdfs:subClassOf <https://w3id.org/skgo/modsci#Chemistry> ;
                                                       rdfs:comment "Organometallic chemistry is the study of chemical compounds containing bonds between carbon and a metal." ;
                                                       rdfs:label "Organometallic Chemistry" .


###  https://w3id.org/skgo/modsci#Paleoclimatology
<https://w3id.org/skgo/modsci#Paleoclimatology> rdf:type owl:Class ;
                                                rdfs:subClassOf <https://w3id.org/skgo/modsci#EarthScience> ;
                                                rdfs:comment "Paleoclimatology is the study of climates for which systematic measurements were not taken." ;
                                                rdfs:label "Paleoclimatology" .


###  https://w3id.org/skgo/modsci#Paleontology
<https://w3id.org/skgo/modsci#Paleontology> rdf:type owl:Class ;
                                            rdfs:subClassOf <https://w3id.org/skgo/modsci#Biology> ;
                                            rdfs:comment "Paleontology is the study of the developing history of life on earth, of ancient plants and animals based on the fossil record, evidence of their existence preserved in rocks." ;
                                            rdfs:label "Paleontology" .


###  https://w3id.org/skgo/modsci#Palynology
<https://w3id.org/skgo/modsci#Palynology> rdf:type owl:Class ;
                                          rdfs:subClassOf <https://w3id.org/skgo/modsci#EarthScience> ;
                                          rdfs:comment "Palynology is literally the \"study of dust\" or of \"particles that are strewn\"." ;
                                          rdfs:label "Palynology" .


###  https://w3id.org/skgo/modsci#ParallelComputing
<https://w3id.org/skgo/modsci#ParallelComputing> rdf:type owl:Class ;
                                                 rdfs:subClassOf <https://w3id.org/skgo/modsci#DistributedSystems> ;
                                                 rdfs:comment "Parallel computing is a type of computation in which many calculations or the execution of processes are carried out simultaneously." ;
                                                 rdfs:label "Parallel Computing" .


###  https://w3id.org/skgo/modsci#Parasitology
<https://w3id.org/skgo/modsci#Parasitology> rdf:type owl:Class ;
                                            rdfs:subClassOf <https://w3id.org/skgo/modsci#Biology> ;
                                            rdfs:comment "Parasitology is the study of parasites in host organisms, including humans (medical parasitology)." ;
                                            rdfs:label "Parasitology" .


###  https://w3id.org/skgo/modsci#ParticlePhysics
<https://w3id.org/skgo/modsci#ParticlePhysics> rdf:type owl:Class ;
                                               rdfs:subClassOf <https://w3id.org/skgo/modsci#Physics> ;
                                               rdfs:comment "Particle physics is a branch of physics that studies the elementary constituents of matter and radiation, and the interactions between them." ;
                                               rdfs:label "Particle Physics" .


###  https://w3id.org/skgo/modsci#Pharmacology
<https://w3id.org/skgo/modsci#Pharmacology> rdf:type owl:Class ;
                                            rdfs:subClassOf <https://w3id.org/skgo/modsci#Biology> ;
                                            rdfs:comment "Pharmacology is the study of how chemical substances interact with living systems." ;
                                            rdfs:label "Pharmacology" .


###  https://w3id.org/skgo/modsci#Pharmacy
<https://w3id.org/skgo/modsci#Pharmacy> rdf:type owl:Class ;
                                        rdfs:subClassOf <https://w3id.org/skgo/modsci#HealthSciences> ;
                                        rdfs:comment "Pharmacy is the science and technique of preparing, dispensing, and reviewing drugs and providing additional clinical services." ;
                                        rdfs:label "Pharmacy" .


###  https://w3id.org/skgo/modsci#Philosophy
<https://w3id.org/skgo/modsci#Philosophy> rdf:type owl:Class ;
                                          rdfs:subClassOf <https://w3id.org/skgo/modsci#FormalScience> ;
                                          rdfs:comment "Philosophy of science is a branch of philosophy concerned with the foundations, methods, and implications of science." ;
                                          rdfs:label "Philosophy of Science" .


###  https://w3id.org/skgo/modsci#Photochemistry
<https://w3id.org/skgo/modsci#Photochemistry> rdf:type owl:Class ;
                                              rdfs:subClassOf <https://w3id.org/skgo/modsci#Chemistry> ;
                                              rdfs:comment "Photochemistry, a sub-discipline of chemistry, is the study of the interactions between atoms, small molecules, and light (or electromagnetic radiation)." ;
                                              rdfs:label "Photochemistry" .


###  https://w3id.org/skgo/modsci#Phylogeny
<https://w3id.org/skgo/modsci#Phylogeny> rdf:type owl:Class ;
                                         rdfs:subClassOf <https://w3id.org/skgo/modsci#Biology> ;
                                         rdfs:comment "Phylogenetics is the study of the evolutionary history and relationships among individuals or groups of organisms." ;
                                         rdfs:label "Phylogeny" .


###  https://w3id.org/skgo/modsci#PhysicalChemistry
<https://w3id.org/skgo/modsci#PhysicalChemistry> rdf:type owl:Class ;
                                                 rdfs:subClassOf <https://w3id.org/skgo/modsci#Chemistry> ;
                                                 rdfs:comment "Physical chemistry is the study of macroscopic, atomic, subatomic, and particulate phenomena in chemical systems in terms of the principles, practices, and concepts of physics such as motion, energy, force, time, thermodynamics, quantum chemistry, statistical mechanics, analytical dynamics and chemical equilibrium." ;
                                                 rdfs:label "Physical Chemistry" .


###  https://w3id.org/skgo/modsci#PhysicalGeography
<https://w3id.org/skgo/modsci#PhysicalGeography> rdf:type owl:Class ;
                                                 rdfs:subClassOf <https://w3id.org/skgo/modsci#EarthScience> ;
                                                 rdfs:comment "Physical geography is a subfield of geography, closely related to geology, that focuses on the spatial characteristics of natural processes, within the hydrosphere, biosphere, atmosphere and lithosphere." ;
                                                 rdfs:label "Physical Geography" .


###  https://w3id.org/skgo/modsci#Physics
<https://w3id.org/skgo/modsci#Physics> rdf:type owl:Class ;
                                       rdfs:subClassOf <https://w3id.org/skgo/modsci#NaturalScience> ;
                                       rdfs:comment "Physics is the science of the natural world. It deals with matter, energy, and the fundamental forces that govern the interactions between particles." ;
                                       rdfs:label "Physics" .


###  https://w3id.org/skgo/modsci#Physiology
<https://w3id.org/skgo/modsci#Physiology> rdf:type owl:Class ;
                                          rdfs:subClassOf <https://w3id.org/skgo/modsci#Biology> ;
                                          rdfs:comment "Physiology is the branch of science that describes the mechanisms of cell, tissue and organ function in organisms." ;
                                          rdfs:label "Physiology" .


###  https://w3id.org/skgo/modsci#PlanetaryScience
<https://w3id.org/skgo/modsci#PlanetaryScience> rdf:type owl:Class ;
                                                rdfs:subClassOf <https://w3id.org/skgo/modsci#Astronomy> ;
                                                rdfs:comment "Planetary science is a broad field of science that studies all planets." ;
                                                rdfs:label "Planetary Science" .


###  https://w3id.org/skgo/modsci#PlasmaPhysics
<https://w3id.org/skgo/modsci#PlasmaPhysics> rdf:type owl:Class ;
                                             rdfs:subClassOf <https://w3id.org/skgo/modsci#Physics> ;
                                             rdfs:comment "Plasma physics is the study of ionized gases." ;
                                             rdfs:label "Plasma Physics" .


###  https://w3id.org/skgo/modsci#PoliticalEconomy
<https://w3id.org/skgo/modsci#PoliticalEconomy> rdf:type owl:Class ;
                                                rdfs:subClassOf <https://w3id.org/skgo/modsci#InterdisciplinaryStudies> ;
                                                rdfs:comment "Political economy is the study of production and trade and their relations with law, custom and government; and with the distribution of national income and wealth." ;
                                                rdfs:label "Political Economy" .


###  https://w3id.org/skgo/modsci#PoliticalScience
<https://w3id.org/skgo/modsci#PoliticalScience> rdf:type owl:Class ;
                                                rdfs:subClassOf <https://w3id.org/skgo/modsci#SocialSciences> ;
                                                rdfs:comment "Political science is a social science which deals with systems of governance, and the analysis of political activities, political thoughts, and political behavior." ;
                                                rdfs:label "Political Science" .


###  https://w3id.org/skgo/modsci#ProgrammingLanguage
<https://w3id.org/skgo/modsci#ProgrammingLanguage> rdf:type owl:Class ;
                                                   rdfs:subClassOf <https://w3id.org/skgo/modsci#ProgrammingLanguages> ;
                                                   rdfs:comment "A programming language is a formal language, which comprises a set of instructions that produce various kinds of output. Programming languages are used in computer programming to implement algorithms." ;
                                                   rdfs:label "Programming Language" .


###  https://w3id.org/skgo/modsci#ProgrammingLanguageTheory
<https://w3id.org/skgo/modsci#ProgrammingLanguageTheory> rdf:type owl:Class ;
                                                         rdfs:subClassOf <https://w3id.org/skgo/modsci#ProgrammingLanguages> ;
                                                         rdfs:comment "Programming language theory (PLT) is a branch of computer science that deals with the design, implementation, analysis, characterization, and classification of programming languages and their individual features." ;
                                                         rdfs:label "Programming Language Theory" .


###  https://w3id.org/skgo/modsci#ProgrammingLanguages
<https://w3id.org/skgo/modsci#ProgrammingLanguages> rdf:type owl:Class ;
                                                    rdfs:subClassOf <https://w3id.org/skgo/modsci#ComputerScience> ;
                                                    rdfs:label "Programming Languages and Compilers" .


###  https://w3id.org/skgo/modsci#Psychology
<https://w3id.org/skgo/modsci#Psychology> rdf:type owl:Class ;
                                          rdfs:subClassOf <https://w3id.org/skgo/modsci#BehaviouralSciences> ;
                                          rdfs:comment "Psychology is a collection of academic, clinical and industrial disciplines concerned with the explanation and prediction of behavior, thinking, emotions, motivations, relationships, potentials and pathologies." ;
                                          rdfs:label "Psychology" .


###  https://w3id.org/skgo/modsci#QuantumComputing
<https://w3id.org/skgo/modsci#QuantumComputing> rdf:type owl:Class ;
                                                rdfs:subClassOf <https://w3id.org/skgo/modsci#TheoryOfComputation> ;
                                                rdfs:comment "Quantum computing is the use of quantum-mechanical phenomena such as superposition and entanglement to perform computation. A quantum computer is used to perform such computation, which can be implemented theoretically or physically." ;
                                                rdfs:label "Quantum Computing" .


###  https://w3id.org/skgo/modsci#QuantumMechanics
<https://w3id.org/skgo/modsci#QuantumMechanics> rdf:type owl:Class ;
                                                rdfs:subClassOf <https://w3id.org/skgo/modsci#Physics> ;
                                                rdfs:comment "Quantum mechanics (also called quantum physics or quantum theory) is a physical theory that is believed to be the formalism underlying the description of all physical systems." ;
                                                rdfs:label "Quantum Mechanics" .


###  https://w3id.org/skgo/modsci#Radiobiology
<https://w3id.org/skgo/modsci#Radiobiology> rdf:type owl:Class ;
                                            rdfs:subClassOf <https://w3id.org/skgo/modsci#Biology> ;
                                            rdfs:comment "Radiobiology is a field of clinical and basic medical sciences that involves the study of the action of ionizing radiation on living things, especially health effects of radiation." ;
                                            rdfs:label "Radiation Biology" .


###  https://w3id.org/skgo/modsci#Radiochemistry
<https://w3id.org/skgo/modsci#Radiochemistry> rdf:type owl:Class ;
                                              rdfs:subClassOf <https://w3id.org/skgo/modsci#Chemistry> ;
                                              rdfs:comment "Radiochemistry is the chemistry of radioactive materials, where radioactive isotopes of elements are used to study the properties and chemical reactions of non-radioactive isotopes (often within radiochemistry the absence of radioactivity leads to a substance being described as being inactive as the isotopes are stable)." ;
                                              rdfs:label "Radiochemistry" .


###  https://w3id.org/skgo/modsci#RelationalDatabases
<https://w3id.org/skgo/modsci#RelationalDatabases> rdf:type owl:Class ;
                                                   rdfs:subClassOf <https://w3id.org/skgo/modsci#Databases> ;
                                                   rdfs:comment "A relational database is a digital database based on the relational model of data, as proposed by E. F. Codd in 1970." ;
                                                   rdfs:label "Relational Databases" .


###  https://w3id.org/skgo/modsci#ReverseEngineering
<https://w3id.org/skgo/modsci#ReverseEngineering> rdf:type owl:Class ;
                                                  rdfs:subClassOf <https://w3id.org/skgo/modsci#SoftwareEngineering> ;
                                                  rdfs:comment "Reverse engineering, also called back engineering, is the process by which a man-made object is deconstructed to reveal its designs, architecture, or to extract knowledge from the object; similar to scientific research, the only difference being that scientific research is about a natural phenomenon." ;
                                                  rdfs:label "Reverse Engineering" .


###  https://w3id.org/skgo/modsci#ScienceAndTechnologyStudies
<https://w3id.org/skgo/modsci#ScienceAndTechnologyStudies> rdf:type owl:Class ;
                                                           rdfs:subClassOf <https://w3id.org/skgo/modsci#InterdisciplinaryStudies> ;
                                                           rdfs:comment "Science and technology studies is the study of how society, politics, and culture affect scientific research and technological innovation, and how these, in turn, affect society, politics and culture." ;
                                                           rdfs:label "Science and Technology Studies" .


###  https://w3id.org/skgo/modsci#ScienceStudies
<https://w3id.org/skgo/modsci#ScienceStudies> rdf:type owl:Class ;
                                              rdfs:subClassOf <https://w3id.org/skgo/modsci#InterdisciplinaryStudies> ;
                                              rdfs:comment "Science studies is an interdisciplinary research area that seeks to situate scientific expertise in broad social, historical, and philosophical contexts." ;
                                              rdfs:label "Science Studies" .


###  https://w3id.org/skgo/modsci#ScientificDiscovery
<https://w3id.org/skgo/modsci#ScientificDiscovery> rdf:type owl:Class .


###  https://w3id.org/skgo/modsci#ScientificMethod
<https://w3id.org/skgo/modsci#ScientificMethod> rdf:type owl:Class .


###  https://w3id.org/skgo/modsci#ScientificModeling
<https://w3id.org/skgo/modsci#ScientificModeling> rdf:type owl:Class ;
                                                  rdfs:subClassOf <https://w3id.org/skgo/modsci#InterdisciplinaryStudies> ;
                                                  rdfs:comment "Scientific modelling is a scientific activity, the aim of which is to make a particular part or feature of the world easier to understand, define, quantify, visualize, or simulate by referencing it to existing and usually commonly accepted knowledge." ;
                                                  rdfs:label "Scientific Modelling" .


###  https://w3id.org/skgo/modsci#Scientist
<https://w3id.org/skgo/modsci#Scientist> rdf:type owl:Class .


###  https://w3id.org/skgo/modsci#Semantics
<https://w3id.org/skgo/modsci#Semantics> rdf:type owl:Class ;
                                         rdfs:subClassOf <https://w3id.org/skgo/modsci#ProgrammingLanguages> ;
                                         rdfs:comment "In programming language theory, semantics is the field concerned with the rigorous mathematical study of the meaning of programming languages. It does so by evaluating the meaning of syntactically valid strings defined by a specific programming language, showing the computation involved." ;
                                         rdfs:label "Semantics" .


###  https://w3id.org/skgo/modsci#Semiotics
<https://w3id.org/skgo/modsci#Semiotics> rdf:type owl:Class ;
                                         rdfs:subClassOf <https://w3id.org/skgo/modsci#InterdisciplinaryStudies> ,
                                                         <https://w3id.org/skgo/modsci#SocialSciences> ;
                                         rdfs:comment "Semiotics is the study of signs (symbols) and signification systems, or rather semiotics are general theories of signs." ;
                                         rdfs:label "Semiotics" .


###  https://w3id.org/skgo/modsci#SocialPsychology
<https://w3id.org/skgo/modsci#SocialPsychology> rdf:type owl:Class ;
                                                rdfs:subClassOf <https://w3id.org/skgo/modsci#BehaviouralSciences> ;
                                                rdfs:comment "Social psychology is the scientific study of how people's thoughts, feelings, and behaviors are influenced by the actual, imagined or implied presence of others." ;
                                                rdfs:label "Social Psychology" .


###  https://w3id.org/skgo/modsci#SocialSciences
<https://w3id.org/skgo/modsci#SocialSciences> rdf:type owl:Class ;
                                              rdfs:subClassOf <https://w3id.org/skgo/modsci#ModernScience> ;
                                              rdfs:comment "The social sciences are academic disciplines concerned with the study of the social life of human groups and individuals including anthropology, economics, geography, history, political science, psychology, social studies, and sociology." ;
                                              rdfs:label "Social Sciences" .


###  https://w3id.org/skgo/modsci#SocialWork
<https://w3id.org/skgo/modsci#SocialWork> rdf:type owl:Class ;
                                          rdfs:subClassOf <https://w3id.org/skgo/modsci#HealthSciences> ;
                                          rdfs:comment "Social work is an academic discipline and profession that concerns itself with individuals, families, groups and communities in an effort to enhance social functioning and overall well-being." ;
                                          rdfs:label "Social Work" .


###  https://w3id.org/skgo/modsci#Sociobiology
<https://w3id.org/skgo/modsci#Sociobiology> rdf:type owl:Class ;
                                            rdfs:subClassOf <https://w3id.org/skgo/modsci#BehaviouralSciences> ;
                                            rdfs:comment "Sociobiology is a field of biology that aims to examine and explain social behavior in terms of evolution." ;
                                            rdfs:label "Sociobiology" .


###  https://w3id.org/skgo/modsci#Sociology
<https://w3id.org/skgo/modsci#Sociology> rdf:type owl:Class ;
                                         rdfs:subClassOf <https://w3id.org/skgo/modsci#SocialSciences> ;
                                         rdfs:comment "Sociology is the study of social behaviour or society, including its origins, development, organization, networks, and institutions. and critical analysis to develop a body of knowledge about social order, disorder, and change." ;
                                         rdfs:label "Sociology" .


###  https://w3id.org/skgo/modsci#SoftwareEngineering
<https://w3id.org/skgo/modsci#SoftwareEngineering> rdf:type owl:Class ;
                                                   rdfs:subClassOf <https://w3id.org/skgo/modsci#ComputerScience> ;
                                                   rdfs:comment "Software engineering is the application of engineering to the development of software in a systematic method." ;
                                                   rdfs:label "Software Engineering" .


###  https://w3id.org/skgo/modsci#SoilBiology
<https://w3id.org/skgo/modsci#SoilBiology> rdf:type owl:Class ;
                                           rdfs:subClassOf <https://w3id.org/skgo/modsci#Biology> ;
                                           rdfs:comment "Soil biology is the study of microbial and faunal activity and ecology in soil." ;
                                           rdfs:label "Soil Biology" .


###  https://w3id.org/skgo/modsci#SoilScience
<https://w3id.org/skgo/modsci#SoilScience> rdf:type owl:Class ;
                                           rdfs:subClassOf <https://w3id.org/skgo/modsci#EarthScience> ;
                                           rdfs:comment "Soil science is the study of soil as a natural resource on the surface of the Earth including soil formation, classification and mapping; physical, chemical, biological, and fertility properties of soils; and these properties in relation to the use and management of soils." ;
                                           rdfs:label "Soil Science" .


###  https://w3id.org/skgo/modsci#SolidMechanics
<https://w3id.org/skgo/modsci#SolidMechanics> rdf:type owl:Class ;
                                              rdfs:subClassOf <https://w3id.org/skgo/modsci#Physics> ;
                                              rdfs:comment "Solid mechanics is a mathematical discipline within continuum mechanics, dealing with the mechanical behavior of solid materials." ;
                                              rdfs:label "Solid Mechanics" .


###  https://w3id.org/skgo/modsci#SolidStateChemistry
<https://w3id.org/skgo/modsci#SolidStateChemistry> rdf:type owl:Class ;
                                                   rdfs:subClassOf <https://w3id.org/skgo/modsci#Chemistry> ;
                                                   rdfs:comment "Solid-state chemistry, also sometimes referred as materials chemistry, is the study of the synthesis, structure, and properties of solid phase materials, particularly, but not necessarily exclusively of, non-molecular solids." ;
                                                   rdfs:label "Solid-State Chemistry" .


###  https://w3id.org/skgo/modsci#SpaceScience
<https://w3id.org/skgo/modsci#SpaceScience> rdf:type owl:Class ;
                                            rdfs:subClassOf <https://w3id.org/skgo/modsci#EarthScience> ;
                                            rdfs:comment "Space science encompasses all of the scientific disciplines that involve space exploration and study natural phenomena and physical bodies occurring in outer space, such as space medicine and astrobiology." ;
                                            rdfs:label "Space Science" .


###  https://w3id.org/skgo/modsci#SportsScience
<https://w3id.org/skgo/modsci#SportsScience> rdf:type owl:Class ;
                                             rdfs:subClassOf <https://w3id.org/skgo/modsci#AppliedSciences> ;
                                             rdfs:comment "Sports science is a discipline that studies how the healthy human body works during exercise, and how sport and physical activity promote health and performance from cellular to whole body perspectives." ;
                                             rdfs:label "Sports Science" .


###  https://w3id.org/skgo/modsci#Statistics
<https://w3id.org/skgo/modsci#Statistics> rdf:type owl:Class ;
                                          rdfs:subClassOf <https://w3id.org/skgo/modsci#FormalScience> ;
                                          rdfs:comment "Statistics is the discipline that concerns the collection, organization, displaying, analysis, interpretation and presentation of data." ;
                                          rdfs:label "Statistics" .


###  https://w3id.org/skgo/modsci#StellarAstronomy
<https://w3id.org/skgo/modsci#StellarAstronomy> rdf:type owl:Class ;
                                                rdfs:subClassOf <https://w3id.org/skgo/modsci#Astronomy> ;
                                                rdfs:comment "The study of stars and stellar evolution is fundamental to our understanding of the Universe." ;
                                                rdfs:label "Stellar Astronomy" .


###  https://w3id.org/skgo/modsci#Stereochemistry
<https://w3id.org/skgo/modsci#Stereochemistry> rdf:type owl:Class ;
                                               rdfs:subClassOf <https://w3id.org/skgo/modsci#Chemistry> ;
                                               rdfs:comment "Stereochemistry, a subdiscipline of chemistry, involves the study of the relative spatial arrangement of atoms that form the structure of molecules and their manipulation." ;
                                               rdfs:label "Stereochemistry" .


###  https://w3id.org/skgo/modsci#StructuredStorage
<https://w3id.org/skgo/modsci#StructuredStorage> rdf:type owl:Class ;
                                                 rdfs:subClassOf <https://w3id.org/skgo/modsci#Databases> ;
                                                 rdfs:comment "Structured storage is computer storage for structured data, often in the form of a distributed database." ;
                                                 rdfs:label "Structured Storage" .


###  https://w3id.org/skgo/modsci#SupramolecularChemistry
<https://w3id.org/skgo/modsci#SupramolecularChemistry> rdf:type owl:Class ;
                                                       rdfs:subClassOf <https://w3id.org/skgo/modsci#Chemistry> ;
                                                       rdfs:comment "Supramolecular chemistry is a branch of chemistry that describes self-organization or self-assembly of systems to well-defined molecular architectures." ;
                                                       rdfs:label "Supramolecular Chemistry" .


###  https://w3id.org/skgo/modsci#SurfaceChemistry
<https://w3id.org/skgo/modsci#SurfaceChemistry> rdf:type owl:Class ;
                                                rdfs:subClassOf <https://w3id.org/skgo/modsci#Chemistry> ;
                                                rdfs:comment "Surface chemistry is the study of chemical phenomena that occur at the interface of two phases" ;
                                                rdfs:label "Surface Chemistry" .


###  https://w3id.org/skgo/modsci#SystemsScience
<https://w3id.org/skgo/modsci#SystemsScience> rdf:type owl:Class ;
                                              rdfs:subClassOf <https://w3id.org/skgo/modsci#InterdisciplinaryStudies> ;
                                              rdfs:comment "Systems science is the field of science surrounding systems theory, cybernetics, the science of complex systems." ;
                                              rdfs:label "Systems Science" .


###  https://w3id.org/skgo/modsci#Technology
<https://w3id.org/skgo/modsci#Technology> rdf:type owl:Class ;
                                          rdfs:subClassOf <https://w3id.org/skgo/modsci#FormalScience> ;
                                          rdfs:comment "Technology is the collection of techniques, skills, methods, and processes used in the production of goods or services or in the accomplishment of objectives, such as scientific investigation." ;
                                          rdfs:label "Technology" .


###  https://w3id.org/skgo/modsci#TheoreticalBiology
<https://w3id.org/skgo/modsci#TheoreticalBiology> rdf:type owl:Class ;
                                                  rdfs:subClassOf <https://w3id.org/skgo/modsci#Biology> ;
                                                  rdfs:comment "Theoretical biology is a branch of biology which employs theoretical analysis, mathematical models and abstractions of the living organisms to investigate the principles that govern the structure, development and behavior of the systems" ;
                                                  rdfs:label "Theoretical Biology" .


###  https://w3id.org/skgo/modsci#TheoreticalChemistry
<https://w3id.org/skgo/modsci#TheoreticalChemistry> rdf:type owl:Class ;
                                                    rdfs:subClassOf <https://w3id.org/skgo/modsci#Chemistry> ;
                                                    rdfs:comment "Theoretical chemistry is the application of theoretical reasoning to chemistry." ;
                                                    rdfs:label "Theoretical Chemistry" .


###  https://w3id.org/skgo/modsci#TheoreticalLinguistics
<https://w3id.org/skgo/modsci#TheoreticalLinguistics> rdf:type owl:Class ;
                                                      rdfs:subClassOf <https://w3id.org/skgo/modsci#FormalScience> ;
                                                      rdfs:comment "Theoretical linguistics, or general linguistics, is the branch of linguistics which inquires into the nature of language itself and seeks to answer fundamental questions as to what language is; how it works; how universal grammar (UG) as a domain-specific mental organ operates, if it exists at all; what are its unique properties; how does language relate to other cognitive processes, etc." ;
                                                      rdfs:label "Theoretical Linguistics" .


###  https://w3id.org/skgo/modsci#TheoryOfComputation
<https://w3id.org/skgo/modsci#TheoryOfComputation> rdf:type owl:Class ;
                                                   rdfs:subClassOf <https://w3id.org/skgo/modsci#ComputerScience> ;
                                                   rdfs:label "Theory of Computation" .


###  https://w3id.org/skgo/modsci#Thermodynamics
<https://w3id.org/skgo/modsci#Thermodynamics> rdf:type owl:Class ;
                                              rdfs:subClassOf <https://w3id.org/skgo/modsci#Physics> ;
                                              rdfs:comment "Thermodynamics concerns the physics of heat, work, temperature, energy, and entropy." ;
                                              rdfs:label "Thermodynamics" .


###  https://w3id.org/skgo/modsci#Toxicology
<https://w3id.org/skgo/modsci#Toxicology> rdf:type owl:Class ;
                                          rdfs:subClassOf <https://w3id.org/skgo/modsci#Biology> ;
                                          rdfs:comment "Toxicology is a scientific discipline, overlapping with biology, chemistry, pharmacology, and medicine, that involves the study of the adverse effects of chemical substances on living organisms and the practice of diagnosing and treating exposures to toxins and toxicants." ;
                                          rdfs:label "Toxicology" .


###  https://w3id.org/skgo/modsci#Transdisciplinarity
<https://w3id.org/skgo/modsci#Transdisciplinarity> rdf:type owl:Class ;
                                                   rdfs:subClassOf <https://w3id.org/skgo/modsci#InterdisciplinaryStudies> ;
                                                   rdfs:comment "Transdisciplinarity connotes a research strategy that crosses many disciplinary boundaries to create a holistic approach." ;
                                                   rdfs:label "Transdisciplinarity" .


###  https://w3id.org/skgo/modsci#TypeTheory
<https://w3id.org/skgo/modsci#TypeTheory> rdf:type owl:Class ;
                                          rdfs:subClassOf <https://w3id.org/skgo/modsci#ProgrammingLanguages> ;
                                          rdfs:comment "In mathematics, logic, and computer science, a type theory is any of a class of formal systems, some of which can serve as alternatives to set theory as a foundation for all mathematics. In type theory, every \"term\" has a \"type\" and operations are restricted to terms of a certain type." ;
                                          rdfs:label "Type Theory" .


###  https://w3id.org/skgo/modsci#UrbanPlanning
<https://w3id.org/skgo/modsci#UrbanPlanning> rdf:type owl:Class ;
                                             rdfs:subClassOf <https://w3id.org/skgo/modsci#InterdisciplinaryStudies> ;
                                             rdfs:comment "Urban planning is a technical and political process concerned with the development and design of land use and the built environment, including air, water, and the infrastructure passing into and out of urban areas, such as transportation, communications, and distribution networks." ;
                                             rdfs:label "Urban Planning" .


###  https://w3id.org/skgo/modsci#VeterinaryMedicine
<https://w3id.org/skgo/modsci#VeterinaryMedicine> rdf:type owl:Class ;
                                                  rdfs:subClassOf <https://w3id.org/skgo/modsci#HealthSciences> ;
                                                  rdfs:comment "Veterinary medicine is the branch of medicine that deals with the prevention, diagnosis and treatment of disease, disorder and injury in animals." ;
                                                  rdfs:label "Veterinary Medicine" .


###  https://w3id.org/skgo/modsci#Volcanology
<https://w3id.org/skgo/modsci#Volcanology> rdf:type owl:Class ;
                                           rdfs:subClassOf <https://w3id.org/skgo/modsci#EarthScience> ;
                                           rdfs:comment "Volcanology is a branch of geology that deals with the study of volcanoes, lava, magma, and related geological phenomena." ;
                                           rdfs:label "Volcanology" .


###  https://w3id.org/skgo/modsci#Zoology
<https://w3id.org/skgo/modsci#Zoology> rdf:type owl:Class ;
                                       rdfs:subClassOf <https://w3id.org/skgo/modsci#Biology> ;
                                       rdfs:comment "Zoology is the study of the biology of animals." ;
                                       rdfs:label "Zoology" .


###  Generated by the OWL API (version 4.5.9.2019-02-01T07:24:44Z) https://github.com/owlcs/owlapi
